Subst.v
@@ -13,15 +13,12 @@ Inductive eval_name : term -> term -> Prop :=
   | eval_name_let ts t v :
       eval_name (subst (scat (map (Let ts) ts) Var) t) v ->
       eval_name (Let ts t) v
-  | eval_name_ctor c ts :
-      eval_name (Ctor c ts) (Ctor c ts)
+  | eval_name_cons c ts :
+      eval_name (Cons c ts) (Cons c ts)
   | eval_name_case c i t t0 ts pts v :
-      eval_name t (Ctor c ts) ->
-      ( forall d, nth d pts i = (c, size ts, t0) ) ->
-      ( forall j, j < i ->
-        forall d t0, 
-        nth d pts j = (c, size ts, t0) ->
-        False ) ->
+      eval_name t (Cons c ts) ->
+      (forall d, nth d pts i = (c, size ts, t0)) ->
+      (forall j d t0, nth d pts j = (c, size ts, t0) -> i <= j) ->
       eval_name (subst (scat ts Var) t0) v ->
       eval_name (Case t pts) v.
 
@@ -29,7 +26,7 @@ CoInductive diverge_name : term -> Prop :=
   | diverge_name_appL t1 t2 :
       diverge_name t1 ->
       diverge_name (App t1 t2)
-  | diverge_name_appabs t0 t1 t2 :
+  | diverge_name_beta t0 t1 t2 :
       eval_name t1 (Abs t0) ->
       diverge_name (subst (scons t2 Var) t0) ->
       diverge_name (App t1 t2)
@@ -40,55 +37,64 @@ CoInductive diverge_name : term -> Prop :=
       diverge_name t ->
       diverge_name (Case t pts)
   | diverge_name_casematch c i t t0 ts pts :
-      eval_name t (Ctor c ts) ->
-      ( forall d, nth d pts i = (c, size ts, t0) ) ->
-      ( forall j, j < i ->
-        forall d t0, 
-        nth d pts j = (c, size ts, t0) ->
-        False ) ->
+      eval_name t (Cons c ts) ->
+      (forall d, nth d pts i = (c, size ts, t0)) ->
+      (forall j d t0, nth d pts j = (c, size ts, t0) -> i <= j) ->
       diverge_name (subst (scat ts Var) t0) ->
       diverge_name (Case t pts).
 
 Hint Constructors eval_name diverge_name.
 
 Inductive corr_term (P : nat -> Prop) :
-      (nat -> term) -> term -> term -> Prop :=
-  | corr_term_loc mu l t' :
+      seq (option term) -> (nat -> term) -> term -> term -> Prop :=
+  | corr_term_indir H mu l t t' :
+      nth None H l = Some t ->
+      corr_term P H mu t t' ->
+      corr_term P H mu (Loc l) t'
+  | corr_term_loc H mu l t' :
       P l ->
       mu l = t' ->
-      corr_term P mu (Loc l) t'
-  | corr_term_var mu x :
-      corr_term P mu (Var x) (Var x)
-  | corr_term_abs mu t t' :
-      corr_term P (rename succn \o mu) t t' ->
-      corr_term P mu (Abs t) (Abs t')
-  | corr_term_app mu t1 t1' t2 t2' :
-      corr_term P mu t1 t1' ->
-      corr_term P mu t2 t2' ->
-      corr_term P mu (App t1 t2) (App t1' t2')
-  | corr_term_let mu ts ts' t t' :
+      corr_term P H mu (Loc l) t'
+  | corr_term_var H mu x :
+      corr_term P H mu (Var x) (Var x)
+  | corr_term_abs H mu t t' :
+      corr_term P (map (omap (rename succn)) H) (rename succn \o mu) t t' ->
+      corr_term P H mu (Abs t) (Abs t')
+  | corr_term_app H mu t1 t1' t2 t2' :
+      corr_term P H mu t1 t1' ->
+      corr_term P H mu t2 t2' ->
+      corr_term P H mu (App t1 t2) (App t1' t2')
+  | corr_term_let H mu ts ts' t t' :
       size ts = size ts' ->
       ( forall x, x < size ts -> forall d,
         corr_term P
+          (map (omap (rename (addn (size ts)))) H)
           (rename (addn (size ts)) \o mu)
           (nth d ts x) (nth d ts' x) ) ->
       corr_term P
+        (map (omap (rename (addn (size ts)))) H)
         (rename (addn (size ts)) \o mu) t t' ->
-      corr_term P mu (Let ts t) (Let ts' t')
-  | corr_term_ctor mu c ts ts' :
+      corr_term P H mu (Let ts t) (Let ts' t')
+  | corr_term_vcons H mu c ls ts' :
+      size ls = size ts' ->
+      ( forall x, x < size ls -> forall d d',
+        corr_term P H mu (Loc (nth d ls x)) (nth d' ts' x) ) ->
+      corr_term P H mu (VCons c ls) (Cons c ts')
+  | corr_term_cons H mu c ts ts' :
       size ts = size ts' ->
       ( forall x, x < size ts -> forall d,
-        corr_term P mu (nth d ts x) (nth d ts' x) ) ->
-      corr_term P mu (Ctor c ts) (Ctor c ts')
-  | corr_term_case mu t t' (pts pts' : seq (ctor * nat * term)) :
-      corr_term P mu t t' ->
+        corr_term P H mu (nth d ts x) (nth d ts' x) ) ->
+      corr_term P H mu (Cons c ts) (Cons c ts')
+  | corr_term_case H mu t t' (pts pts' : seq (cons * nat * term)) :
+      corr_term P H mu t t' ->
       size pts = size pts' ->
       ( forall x d, (nth d pts x).1 = (nth d pts' x).1 ) ->
       ( forall x, x < size pts -> forall d,
         corr_term P
+          (map (omap (rename (addn (nth d pts x).1.2))) H)
           (rename (addn (nth d pts x).1.2) \o mu)
           (nth d pts x).2 (nth d pts' x).2 ) ->
-      corr_term P mu (Case t pts) (Case t' pts').
+      corr_term P H mu (Case t pts) (Case t' pts').
 
 Hint Constructors corr_term.
 
@@ -96,7 +102,7 @@ Definition corr_heap_segment (P P' : nat -> Prop) H mu :=
   forall l, P l ->
   exists t, nth None H l = Some t /\
   exists ts' t', mu l = Let ts' t' /\
-  corr_term P' mu t (subst (scat (map (Let ts') ts') Var) t').
+  corr_term P' H mu t (subst (scat (map (Let ts') ts') Var) t').
 Definition corr_heap P := corr_heap_segment P P.
 
 Lemma eq_omap A B (f g : A -> B) : forall o,
@@ -111,113 +117,198 @@ Lemma omap_comp A B C (f : B -> C) (g : A -> B) : forall o,
   omap f (omap g o) = omap (f \o g) o.
 Proof. by move => [ ]. Qed.
 
-Lemma corr_term_impl P mu t t' :
-  corr_term P mu t t' ->
-  forall (P' : nat -> Prop) mu',
+Lemma nth_map_heap A B H l (f : A -> B) :
+  nth None (map (omap f) H) l = omap f (nth None H l).
+Proof.
+  case (leqP (size H) l) => ?.
+  - by rewrite !nth_default ?size_map.
+  - exact: nth_map.
+Qed.
+
+Lemma corr_term_impl P H mu t t' :
+  corr_term P H mu t t' ->
+  forall (P' : nat -> Prop) H' mu',
   ( forall l, P l -> P' l ) ->
+  ( forall l,
+    nth None H l = None \/
+    nth None H l = nth None H' l ) ->
   ( forall l, P l -> mu l = mu' l ) ->
-  corr_term P' mu' t t'.
+  corr_term P' H' mu' t t'.
 Proof.
-  induction 1 => ? ? HP HPmu; constructor; eauto.
-  - by rewrite -H0 (HPmu _ H).
-  - ( apply: IHcorr_term; eauto ) => l.
-    by move => /HPmu /= ->.
-  - move => ? ? ?.
-    ( apply: H1; eauto ) => l.
-    by move => /HPmu /= ->.
-  - ( apply: IHcorr_term; eauto ) => l.
-    by move => /HPmu /= ->.
-  - move => ? ? ?.
-    ( apply: H3; eauto ) => l.
-    by move => /HPmu /= ->.
-Qed.
-
-Lemma corr_term_rename P mu t t' :
-  corr_term P mu t t' ->
-  forall mu' r,
-  (forall l, mu' l = rename r (mu l)) ->
-  corr_term P mu' (rename r t) (rename r t').
-Proof.
-  induction 1 => ? ? Hmu /=; constructor; rewrite ?size_map; eauto.
-  - by rewrite -H0.
-  - apply: IHcorr_term => ?.
-    rewrite /funcomp Hmu !rename_rename_comp.
-    exact: eq_rename.
-  - move => ? ? d.
-    rewrite !(nth_map d) -?H => //.
-    apply: H1 => // ?.
-    rewrite /funcomp Hmu !rename_rename_comp.
-    apply: eq_rename => ? /=.
-    by rewrite upnren_unfold ltnNge leq_addr addKn.
-  - rewrite -H.
-    apply: IHcorr_term => ?.
-    rewrite /funcomp Hmu !rename_rename_comp.
-    apply: eq_rename => ? /=.
-    by rewrite upnren_unfold ltnNge leq_addr addKn.
-  - move => ? ? d.
-    rewrite !(nth_map d) -?H => //.
-    apply: H1 => // ?.
-  - move => x d.
-    case (leqP (size pts) x) => ?.
-    + rewrite !nth_default ?size_map; congruence.
-    + rewrite !(nth_map d) => /=; congruence.
-  - move => ? ? d.
-    rewrite !(nth_map d) -?H0 ?H1 => //.
-    apply: H3 => // ?.
-    rewrite /funcomp Hmu !rename_rename_comp.
-    apply: eq_rename => ? /=.
-    by rewrite H1 upnren_unfold ltnNge leq_addr addKn.
-Qed.
-
-Lemma corr_term_subst P mu t t' :
-  corr_term P mu t t' ->
-  forall mu' s s',
-  (forall x, corr_term P mu' (s x) (s' x)) ->
-  (forall l, mu' l = subst s' (mu l)) ->
-  corr_term P mu' (subst s t) (subst s' t').
-Proof.
-  induction 1 => ? ? ? Hs Hmu /=; eauto.
+  induction 1 => ? H' ? HP HQ HPmu; eauto.
+  - apply: corr_term_indir; eauto.
+    by move: H0 (HQ l) => -> [ ].
   - apply: corr_term_loc; eauto.
-    by rewrite Hmu H0.
+    erewrite <- HPmu; eauto.
   - constructor.
-    apply: IHcorr_term => [ [ | ? ] //= | ? ].
-    + apply: corr_term_rename; eauto.
+    ( apply: IHcorr_term; eauto ) => l.
+    + rewrite !nth_map_heap.
+      case (HQ l) => ->; eauto.
+    + by move => /HPmu /= ->.
+  - constructor; eauto.
+    + move => ? ? ?.
+      ( apply: H2; eauto ) => l.
+      * rewrite !nth_map_heap.
+        case (HQ l) => ->; eauto.
+      * by move => /HPmu /= ->.
+    + ( apply: IHcorr_term; eauto ) => l.
+      * rewrite !nth_map_heap.
+        case (HQ l) => ->; eauto.
+      * by move => /HPmu /= ->.
+  - constructor; eauto.
+    move => ? ? ?.
+    ( apply: H4; eauto ) => l.
+    + rewrite !nth_map_heap.
+      case (HQ l) => ->; eauto.
+    + by move => /HPmu /= ->.
+Qed.
+
+Lemma corr_term_rename P H mu t t' :
+  corr_term P H mu t t' ->
+  forall H' mu' r,
+  (forall l, mu' l = rename r (mu l)) ->
+  (forall l, nth None H' l = omap (rename r) (nth None H l)) ->
+  corr_term P H' mu' (rename r t) (rename r t').
+Proof.
+  induction 1 => H' ? ? Hmu Hnth /=; eauto.
+  - apply: corr_term_indir; eauto.
+    by rewrite Hnth H0.
+  - apply: corr_term_loc; eauto.
+    by rewrite Hmu H1.
+  - constructor.
+    apply: IHcorr_term => ?.
+    + rewrite /funcomp Hmu !rename_rename_comp.
+      exact: eq_rename.
+    + rewrite !nth_map_heap Hnth !omap_comp.
+      apply: eq_omap => ?.
+      rewrite /funcomp !rename_rename_comp.
+      exact: eq_rename.
+  - constructor; rewrite !size_map -?H0; eauto.
+    + move => ? ? d.
+      rewrite !(nth_map d) -?H0 => //.
+      apply: H2 => // ?.
+      * rewrite /funcomp Hmu !rename_rename_comp.
+        apply: eq_rename => ? /=.
+        by rewrite upnren_unfold ltnNge leq_addr addKn.
+      * rewrite !nth_map_heap Hnth !omap_comp.
+        apply: eq_omap => ?.
+        rewrite /funcomp !rename_rename_comp.
+        apply: eq_rename => x /=.
+        by rewrite upnren_unfold ltnNge leq_addr addKn.
+    + apply: IHcorr_term => ?.
+      * rewrite /funcomp Hmu !rename_rename_comp.
+        apply: eq_rename => ? /=.
+        by rewrite upnren_unfold ltnNge leq_addr addKn.
+      * rewrite !nth_map_heap Hnth !omap_comp.
+        apply: eq_omap => ?.
+        rewrite /funcomp !rename_rename_comp.
+        apply: eq_rename => ? /=.
+        by rewrite upnren_unfold ltnNge leq_addr addKn.
+  - constructor; rewrite ?size_map; eauto.
+    move => ? ? ? d'.
+    rewrite (nth_map d') -?H0 => //.
+    exact: H2.
+  - constructor; rewrite !size_map; eauto.
+    move => ? ? d.
+    rewrite !(nth_map d) -?H0 => //.
+    exact: H2.
+  - constructor; rewrite ?size_map; eauto.
+    + move => x d.
+      case (leqP (size pts) x) => ?.
+      * rewrite !nth_default ?size_map; congruence.
+      * rewrite !(nth_map d) => /=; congruence.
+    + move => ? ? d.
+      rewrite !(nth_map d) -?H1 ?H2 => //.
+      apply: H4 => // ?.
+      * rewrite /funcomp Hmu !rename_rename_comp.
+        apply: eq_rename => x /=.
+        by rewrite upnren_unfold ltnNge H2 leq_addr addKn.
+      * rewrite !nth_map_heap Hnth !omap_comp.
+        apply: eq_omap => ?.
+        rewrite /funcomp !rename_rename_comp.
+        apply: eq_rename => ? /=.
+        by rewrite upnren_unfold ltnNge H2 leq_addr addKn.
+Qed.
+
+Lemma corr_term_subst P H mu t t' :
+  corr_term P H mu t t' ->
+  forall H' mu' s s',
+  (forall x, corr_term P H' mu' (s x) (s' x)) ->
+  (forall l, nth None H' l = omap (subst s) (nth None H l)) ->
+  (forall l, mu' l = subst s' (mu l)) ->
+  corr_term P H' mu' (subst s t) (subst s' t').
+Proof.
+  induction 1 => ? ? ? ? Hs Hnth Hmu /=; eauto.
+  - apply: corr_term_indir; eauto.
+    by rewrite Hnth H0.
+  - apply: corr_term_loc; eauto.
+    by rewrite Hmu H1.
+  - constructor.
+    apply: IHcorr_term => [ [ | ? ] //= | ? | ? ].
+    + ( apply: corr_term_rename; eauto ) => ?.
+      by rewrite nth_map_heap.
+    + rewrite !nth_map_heap Hnth !omap_comp.
+      apply: eq_omap => ?.
+      rewrite /funcomp rename_subst_comp subst_rename_comp.
+      exact: eq_subst.
     + rewrite /funcomp Hmu rename_subst_comp subst_rename_comp.
       exact: eq_subst.
-  - constructor; rewrite !size_map -?H; eauto.
+  - constructor; rewrite !size_map -?H0; eauto.
     + move => ? ? d.
-      rewrite !(nth_map d) -?H => //.
-      apply: H1 => // x.
+      rewrite !(nth_map d) -?H0 => //.
+      apply: H2 => // x.
       * rewrite !upn_unfold.
         case (leqP (size ts) x) => ? //.
-        apply: corr_term_rename; eauto.
+        ( apply: corr_term_rename; eauto ) => ?.
+        by rewrite nth_map_heap.
+      * rewrite !nth_map_heap Hnth !omap_comp.
+        apply: eq_omap => ?.
+        rewrite /funcomp rename_subst_comp subst_rename_comp.
+        apply: eq_subst => ?.
+        by rewrite /funcomp upn_unfold ltnNge leq_addr addKn.
       * rewrite /funcomp Hmu rename_subst_comp subst_rename_comp.
         apply: eq_subst => ?.
         by rewrite /funcomp upn_unfold ltnNge leq_addr addKn.
     + apply IHcorr_term => x.
       * rewrite !upn_unfold.
         case (leqP (size ts) x) => ? //.
-        apply: corr_term_rename; eauto.
+        ( apply: corr_term_rename; eauto ) => ?.
+        by rewrite nth_map_heap.
+      * rewrite !nth_map_heap Hnth !omap_comp.
+        apply: eq_omap => ?.
+        rewrite /funcomp rename_subst_comp subst_rename_comp.
+        apply: eq_subst => ?.
+        by rewrite /funcomp upn_unfold ltnNge leq_addr addKn.
       * rewrite /funcomp Hmu rename_subst_comp subst_rename_comp.
         apply: eq_subst => ?.
         by rewrite /funcomp upn_unfold ltnNge leq_addr addKn.
-  - constructor; rewrite ?size_map -?H; eauto.
-    move => ? ? d.
-    rewrite !(nth_map d) -?H; eauto.
   - constructor; rewrite ?size_map -?H0; eauto.
+    move => ? ? ? d'.
+    rewrite (nth_map d') -?H0 => //.
+    exact: H2.
+  - constructor; rewrite !size_map; eauto.
+    move => ? ? d.
+    rewrite !(nth_map d) -?H0; eauto.
+  - constructor; rewrite ?size_map -?H1; eauto.
     + move => x d.
       case (leqP (size pts) x) => ?.
       * rewrite !nth_default ?size_map; congruence.
       * rewrite !(nth_map d) => /=; congruence.
     + move => i ? d.
-      rewrite !(nth_map d) -?H0 ?H1 => //.
-      apply: H3 => // x.
+      rewrite !(nth_map d) -?H1 ?H2 => //.
+      apply: H4 => // x.
       * rewrite !upn_unfold.
         case (leqP (nth d pts' i).1.2 x) => ? //.
-        apply: corr_term_rename; eauto.
+        ( apply: corr_term_rename; eauto ) => ?.
+        by rewrite nth_map_heap.
+      * rewrite !nth_map_heap Hnth !omap_comp.
+        apply: eq_omap => ?.
+        rewrite /funcomp rename_subst_comp subst_rename_comp.
+        apply: eq_subst => ?.
+        by rewrite /funcomp upn_unfold H2 ltnNge leq_addr addKn.
       * rewrite /funcomp Hmu rename_subst_comp subst_rename_comp.
         apply: eq_subst => ?.
-        by rewrite H1 /funcomp upn_unfold ltnNge leq_addr addKn.
+        by rewrite /funcomp upn_unfold H2 ltnNge leq_addr addKn.
 Qed.
 
 Lemma corr_heap_segment_impl P P' H mu :
@@ -232,6 +323,7 @@ Proof.
     [ ? [ /Hnth -> [ ? [ ? [ -> ? ] ] ] ] ].
   repeat (eexists; eauto).
   ( apply: corr_term_impl; eauto ) => l.
+  move: (nth None H l) (Hnth l) => [ ? /(_ _ erefl) | ]; eauto.
 Qed.
 
 Lemma corr_heap_ext P H mu :
@@ -281,64 +373,122 @@ Proof.
   by case (leqP (size H) l) => [ /(nth_default _) -> | ].
 Qed.
 
+Lemma unwind_indirection P H mu t1 t2 :
+  corr_term P H mu t1 t2 ->
+  exists t1',
+  clos_refl_trans _ (fun p p' => Heaps.red_name p.1 p.2 p'.1 p'.2) (H, t1) (H, t1') /\
+  corr_term P H mu t1' t2 /\
+  forall l, t1' = Loc l -> P l /\ mu l = t2.
+Proof.
+  induction 1.
+  - move: IHcorr_term => [ t1' [ ? [ ? ? ] ] ].
+    exists t1'. split; eauto.
+    refine (rt_trans _ _ _ _ _ (rt_step _ _ _ (_, _) _) _) => /=; eauto.
+  - do 3 (eexists; eauto).
+    inversion 1. subst. eauto.
+  - by do 3 (eexists; eauto).
+  - by do 3 (eexists; eauto).
+  - by do 3 (eexists; eauto).
+  - by do 3 (eexists; eauto).
+  - by do 3 (eexists; eauto).
+  - by do 3 (eexists; eauto).
+  - by do 3 (eexists; eauto).
+Qed.
+
 Theorem eval_name_sound H1 H1' t1 v1 :
   Heaps.eval_name H1 t1 H1' v1 ->
   forall P mu t2,
   corr_heap P H1 mu ->
-  corr_term P mu t1 t2 ->
+  corr_term P H1 mu t1 t2 ->
   exists v2,
   eval_name t2 v2 /\
   exists P' mu',
   corr_heap P' H1' mu' /\
-  corr_term P' mu' v1 v2 /\
+  corr_term P' H1' mu' v1 v2 /\
   ( forall l, P l -> P' l ) /\
-  ( forall l, P l -> mu l = mu' l ).
+  ( forall l, P l -> mu l = mu' l ) /\
+  ( forall l t, nth None H1 l = Some t -> mu l = mu' l ).
 Proof.
   induction 1; inversion 2; subst.
-  - move: (H0) (H2 _ H5) => -> [ ? [ ] ].
+  - move: (H0) H6 => ->. inversion 1. subst.
+    exact: IHeval_name.
+  - move: (H0) (H2 _ H6) => -> [ ? [ ] ].
     inversion 1. subst => [ [ ? [ ? [ -> ] ] ]
       /(IHeval_name _ _ _ H2) [ ? [ ? ? ] ] ].
     repeat (eexists; eauto).
-  - move: (IHeval_name1 _ _ _ H2 H7) =>
+  - move: (IHeval_name1 _ _ _ H2 H9) =>
       [ ? [ ? [ P' [ mu' [ Hheap [ ] ] ] ] ] ].
-    inversion 1. subst => [ [ HP' ? ] ].
-    have Hterm' : corr_term P' mu'
-      (subst (scons t2 Var) t0)
+    inversion 1. subst => [ [ HP' [ ? HQmu' ] ] ].
+    have Hterm' : corr_term P'
+      (rcons H' (Some t2)) mu'
+      (subst (scons (Loc (size H')) Var) t0)
       (subst (scons t2' Var) t').
-    { apply: corr_term_subst; eauto.
+    { apply: corr_term_subst.
+      - ( eapply (corr_term_impl _ _ _ _ _ H8 _
+            (map (omap (rename succn)) (rcons H' (Some t2)))
+            (rename succn \o mu')); eauto ) => l.
+        rewrite !nth_map_heap nth_rcons.
+        case (leqP (size H') l) => [ /(nth_default _) -> //= | ]; eauto.
       - move => [ | ? ] //=.
-        apply: corr_term_impl; eauto.
+        apply: corr_term_indir => /=.
+        + by rewrite nth_rcons ltnn eqxx.
+        + ( apply: corr_term_impl; eauto 2 ) => l /=.
+          move: nth_rcons  (nth None H l)
+            (Heaps.eval_name_heap _ _ _ _ H0 l) =>
+              -> [ ? /(_ _ erefl) | ]; eauto.
+          case (leqP (size H') l) => [ /(nth_default _) -> | ? -> ]; eauto.
+      - move => ?.
+        rewrite nth_map_heap omap_comp (eq_omap _ _ _ id) ?omap_id => // ?.
+        by rewrite /funcomp subst_rename_comp (eq_subst _ _ Var) ?subst_id.
       - move => ?.
         by rewrite /funcomp subst_rename_comp (eq_subst _ _ Var) ?subst_id. }
-    move: (IHeval_name2 _ _ _ Hheap Hterm') =>
-      [ ? [ ? [ ? [ ? [ ? [ ? [ ? HPmu'' ] ] ] ] ] ] ].
+    have Hheap' : corr_heap P' (rcons H' (Some t2)) mu'.
+    { refine (corr_heap_segment_impl _ _ _ _
+        (corr_heap_ext _ _ _ Hheap _ _) _ _ _ _ _ _); eauto.
+      move => l.
+      by move: nth_rcons (leqP (size H') l) => -> [ /(nth_default _) -> | ]. }
+    move: (IHeval_name2 _ _ _ Hheap' Hterm') =>
+      [ ? [ ? [ ? [ ? [ ? [ ? [ ? [ HPmu'' HQmu'' ] ] ] ] ] ] ] ].
     repeat (eexists; eauto).
-    move => ? ?.
-    rewrite -HPmu'' => /=; eauto.
+    + move => ? HP.
+      rewrite -HPmu'' => /=; eauto.
+    + move => l t HQ.
+      move: nth_rcons (leqP (size H') l)
+        (Heaps.eval_name_heap _ _ _ _ H0 _ _ HQ) (HQmu'' l t) =>
+          -> [ /(nth_default _) -> // | Hlt ? <- //= ]; eauto.
   - repeat (eexists; eauto).
   - have Hterm' : corr_term
       (fun l => P l \/ size H <= l /\ l - size H < size ts)
+      (H ++ map (@Some _ \o subst (scat (mkseq (Loc \o addn (size H)) (size ts)) Var)) ts)
       (fun l => if l < size H then mu l else nth (mu l) (map (Let ts') ts') (l - size H))
       (subst (scat (mkseq (Loc \o addn (size H)) (size ts)) Var) t)
       (subst (scat (map (Let ts') ts') Var) t').
     { apply: corr_term_subst.
-      - ( eapply (corr_term_impl _ _ _ _ H9 _
+      - ( eapply (corr_term_impl _ _ _ _ _ H11 _
+            (map (omap (rename (addn (size ts))))
+              (H ++ map (@Some _ \o subst (scat (mkseq (Loc \o addn (size H)) (size ts)) Var)) ts))
             (rename (addn (size ts)) \o
               (fun l => if l < size H then mu l else nth (mu l) (map (Let ts') ts') (l - size H)))); eauto ) => l.
-        by move => /(corr_heap_segment_bound _ _ _ _ H1) /= ->.
+        + rewrite !nth_map_heap nth_cat.
+          case (leqP (size H) l) => [ /(nth_default _) -> | ]; eauto.
+        + by move => /(corr_heap_segment_bound _ _ _ _ H1) /= ->.
       - move => x.
-        rewrite !nth_scat size_mkseq size_map -H5.
+        rewrite !nth_scat size_mkseq size_map -H6.
         case (leqP (size ts) x) => ?.
-        + rewrite !nth_default ?size_mkseq ?size_map -?H5; eauto.
+        + rewrite !nth_default ?size_mkseq ?size_map -?H6; eauto.
         + rewrite nth_mkseq => //=.
           apply: corr_term_loc.
           * rewrite leq_addr addKn. eauto.
           * rewrite ltnNge leq_addr addKn.
             apply: set_nth_default.
-            by rewrite size_map -H5.
+            by rewrite size_map -H6.
+      - move => l.
+        rewrite nth_map_heap omap_comp (eq_omap _ _ _ id) ?omap_id => // ?.
+        rewrite /funcomp subst_rename_comp (eq_subst _ _ Var) ?subst_id => // ? /=.
+        by rewrite nth_scat nth_default size_mkseq ?addKn ?leq_addr.
       - move => ?.
         rewrite /funcomp subst_rename_comp (eq_subst _ _ Var) ?subst_id => //= ?.
-        by rewrite nth_scat nth_default size_map -H5 ?addKn ?leq_addr. }
+        by rewrite nth_scat nth_default size_map -H6 ?addKn ?leq_addr. }
     have Hheap' : corr_heap
       (fun l => P l \/ size H <= l /\ l - size H < size ts)
       (H ++ map (@Some _ \o subst (scat (mkseq (Loc \o addn (size H)) (size ts)) Var)) ts)
@@ -352,133 +502,16 @@ Proof.
         rewrite nth_cat ltnNge Hge (nth_map (Var 0)) => //=.
         repeat (eexists; eauto).
         + apply: (nth_map (Var 0)).
-          by rewrite -H5.
-        + apply: corr_term_subst.
-          { ( refine (corr_term_impl _ _ _ _ (H7 _ _ _) _
-              (rename (addn (size ts)) \o
-                (fun l => if l < size H then mu l else nth (mu l) (map (Let ts') ts') (l - size H))) _ _); eauto ) => l.
-            by move => /(corr_heap_segment_bound _ _ _ _ H1) /= ->. }
-          { move => x.
-            case (leqP (size ts) x) => ?.
-            - by rewrite !nth_scat !nth_default ?size_mkseq ?size_map -?H5.
-            - rewrite !nth_scat nth_mkseq ?(nth_map (Var 0)) -?H5 => //.
-              apply: corr_term_loc.
-              + rewrite leq_addr addKn. eauto.
-              + by rewrite ltnNge leq_addr (nth_map (Var 0)) addKn -?H5. }
-          { move => l.
-            rewrite /funcomp subst_rename_comp (eq_subst _ _ Var) ?subst_id => //= ?.
-            by rewrite nth_scat nth_default size_map -H5 ?leq_addr ?addKn. } }
-    move: (IHeval_name _ _ _ Hheap' Hterm') =>
-      [ ? [ ? [ ? [ ? [ ? [ ? [ ? HPmu' ] ] ] ] ] ] ].
-    repeat (eexists; eauto).
-    move => ? ?.
-    rewrite -HPmu'; eauto.
-    erewrite corr_heap_segment_bound; eauto.
-  - repeat (eexists; eauto).
-  - move: (IHeval_name1 _ _ _ H4 H8) => [ ? [ ? [ P' [ mu' [ Hheap' [ ] ] ] ] ] ].
-    inversion 1. subst => [ [ ? HPmu ] ].
-    have Hlt : i < size pts.
-    { move: (leqP (size pts) i) (H1 (c.+1, 0, Var 0)) =>
-        [ /(nth_default _) -> | // ].
-      inversion 1. subst.
-      by move: (PeanoNat.Nat.neq_succ_diag_l _ H10). }
-    have ? : forall d, nth d pts' i = (c, size ts', (nth (0, 0, Var 0) pts' i).2) => [ d | ].
-    { rewrite (surjective_pairing (nth d pts' i)) -H11 -H12 H1.
-      do 2 f_equal. apply: set_nth_default. congruence. }
-    have ? : forall j, j < i -> forall d t1, nth d pts' j = (c, size ts', t1) -> False => [ j Hlt' d | ].
-    { move: (H2 _ Hlt' d).
-      rewrite
-        (surjective_pairing (nth d pts j))
-        (surjective_pairing (nth d pts' j)) H11 H12 => Hcontra.
-      inversion 1. subst.
-      apply: Hcontra. f_equal. eauto. }
-    have Hterm'' : corr_term P' mu'
-      (subst (scat ts Var) t0)
-      (subst (scat ts' Var) (nth (0, 0, Var 0) pts' i).2).
-    { apply: corr_term_subst => [ | x | ? ].
-      - move: H1 (H13 _ Hlt (0, 0, Var 0)) => -> /corr_term_impl.
-        by apply => [ | /= ? /HPmu -> ].
-      - rewrite !nth_scat H12.
-        case (leqP (size ts) x) => ?.
-        + rewrite !nth_default -?H12; eauto.
-        + eauto using corr_term_impl.
-      - rewrite subst_rename_comp (eq_subst _ _ Var) ?subst_id => //= ?.
-        by rewrite nth_scat nth_default -H12 ?addKn ?leq_addr. }
-    move: (IHeval_name2 _ _ _ Hheap' Hterm'') =>
-      [ ? [ ? [ ? [ ? [ ? [ ? [ ? HPmu' ] ] ] ] ] ] ].
-    repeat (eexists; eauto).
-    move => ? ?.
-    erewrite HPmu; eauto.
-Qed.
-
-Theorem diverge_name_sound :
-  forall H1 t1,
-  Heaps.diverge_name H1 t1 ->
-  forall P mu t2,
-  corr_heap P H1 mu ->
-  corr_term P mu t1 t2 ->
-  diverge_name t2.
-Proof.
-  cofix diverge_name_sound.
-  inversion 1; subst; inversion 2; subst.
-  - move: (H2) (H0 _ H6) => -> [ ? [ ] ].
-    inversion 1. subst => [ [ ? [ ? [ -> ? ] ] ] ].
-    apply: diverge_name_let. eauto.
-  - apply: diverge_name_appL. eauto.
-  - move: (eval_name_sound _ _ _ _ H2 _ _ _ H0 H8) =>
-      [ ? [ ? [ P' [ mu' [ Hheap [ ] ] ] ] ] ].
-    inversion 1. subst => [ [ ? HPmu ] ].
-    have Hterm' : corr_term P' mu'
-      (subst (scons t3 Var) t0)
-      (subst (scons t2' Var) t').
-    { apply: corr_term_subst; eauto.
-      - move => [ | ? ] //=.
-        apply: corr_term_impl; eauto.
-      - move => ?.
-        by rewrite /funcomp subst_rename_comp (eq_subst _ _ Var) ?subst_id. }
-    apply: diverge_name_appabs; eauto.
-  - have Hterm' : corr_term
-      (fun l => P l \/ size H1 <= l /\ l - size H1 < size ts)
-      (fun l => if l < size H1 then mu l else nth (mu l) (map (Let ts') ts') (l - size H1))
-      (subst (scat (mkseq (Loc \o addn (size H1)) (size ts)) Var) t)
-      (subst (scat (map (Let ts') ts') Var) t').
-    { apply: corr_term_subst.
-      - ( eapply (corr_term_impl _ _ _ _ H10 _
-            (rename (addn (size ts)) \o
-              (fun l => if l < size H1 then mu l else nth (mu l) (map (Let ts') ts') (l - size H1)))); eauto ) => l.
-        by move => /(corr_heap_segment_bound _ _ _ _ H0) /= ->.
-      - move => x.
-        rewrite !nth_scat size_mkseq size_map -H6.
-        case (leqP (size ts) x) => ?.
-        + rewrite !nth_default ?size_mkseq ?size_map -?H6; eauto.
-        + rewrite nth_mkseq => //=.
-          apply: corr_term_loc.
-          * rewrite leq_addr addKn. eauto.
-          * rewrite ltnNge leq_addr addKn.
-            apply: set_nth_default.
-            by rewrite size_map -H6.
-      - move => ?.
-        rewrite /funcomp subst_rename_comp (eq_subst _ _ Var) ?subst_id => //= ?.
-        by rewrite nth_scat nth_default size_map -H6 ?addKn ?leq_addr. }
-    have Hheap' : corr_heap
-      (fun l => P l \/ size H1 <= l /\ l - size H1 < size ts)
-      (H1 ++ map (@Some _ \o subst (scat (mkseq (Loc \o addn (size H1)) (size ts)) Var)) ts)
-      (fun l => if l < size H1 then mu l else nth (mu l) (map (Let ts') ts') (l - size H1)).
-    { apply: corr_heap_segment_union.
-      - ( refine (corr_heap_segment_impl _ _ _ _
-          (corr_heap_ext _ _ _ H0 _ _) _ _ _ _ _ _); eauto ) => l.
-        + by move => /(corr_heap_segment_bound _ _ _ _ H0) ->.
-        + by move: nth_cat (leqP (size H1) l) => -> [ /(nth_default _) -> | ].
-      - move => ? [ Hge Hlt ].
-        rewrite nth_cat ltnNge Hge (nth_map (Var 0)) => //=.
-        repeat (eexists; eauto).
-        + apply: (nth_map (Var 0)).
           by rewrite -H6.
         + apply: corr_term_subst.
-          { ( refine (corr_term_impl _ _ _ _ (H8 _ _ _) _
+          { ( refine (corr_term_impl _ _ _ _ _ (H9 _ _ _) _
+              (map (omap (rename (addn (size ts))))
+                (H ++ map (@Some _ \o subst (scat (mkseq (Loc \o addn (size H)) (size ts)) Var)) ts))
               (rename (addn (size ts)) \o
-                (fun l => if l < size H1 then mu l else nth (mu l) (map (Let ts') ts') (l - size H1))) _ _); eauto ) => l.
-            by move => /(corr_heap_segment_bound _ _ _ _ H0) /= ->. }
+                (fun l => if l < size H then mu l else nth (mu l) (map (Let ts') ts') (l - size H))) _ _ _); eauto ) => l.
+            - rewrite !nth_map_heap nth_cat.
+              case (leqP (size H) l) => [ /(nth_default _) -> | ]; eauto.
+            - by move => /(corr_heap_segment_bound _ _ _ _ H1) /= ->. }
           { move => x.
             case (leqP (size ts) x) => ?.
             - by rewrite !nth_scat !nth_default ?size_mkseq ?size_map -?H6.
@@ -487,94 +520,156 @@ Proof.
               + rewrite leq_addr addKn. eauto.
               + by rewrite ltnNge leq_addr (nth_map (Var 0)) addKn -?H6. }
           { move => l.
+            rewrite nth_map_heap omap_comp (eq_omap _ _ _ id) ?omap_id => // ?.
+            rewrite /funcomp subst_rename_comp (eq_subst _ _ Var) ?subst_id => //= ?.
+            by rewrite nth_scat nth_default size_mkseq ?leq_addr ?addKn. }
+          { move => l.
             rewrite /funcomp subst_rename_comp (eq_subst _ _ Var) ?subst_id => //= ?.
             by rewrite nth_scat nth_default size_map -H6 ?leq_addr ?addKn. } }
-    apply: diverge_name_let. eauto.
-  - apply: diverge_name_case. eauto.
-  - move: (eval_name_sound _ _ _ _ H2 _ _ _ H0 H9) => [ ? [ ? [ P' [ mu' [ Hheap' [ ] ] ] ] ] ].
-    inversion 1. subst => [ [ ? HPmu ] ].
+    move: (IHeval_name _ _ _ Hheap' Hterm') =>
+      [ ? [ ? [ ? [ ? [ ? [ ? [ ? [ HPmu' HQmu' ] ] ] ] ] ] ] ].
+    repeat (eexists; eauto).
+    + move => ? HP.
+      rewrite -HPmu'; eauto.
+      erewrite corr_heap_segment_bound; eauto.
+    + move => l t_.
+      by move: nth_cat (leqP (size H) l) (HQmu' l t_) =>
+        -> [ /(nth_default _) -> | ].
+  - repeat (eexists; eauto).
+  - do 2 (eexists; eauto).
+    exists P, mu. split.
+    { move => l /H0 [ ? [ ] ].
+      move: nth_cat (leqP (size H) l) =>
+        -> [ /(nth_default _) -> //
+           | ? -> [ ? [ ? [ -> Hterm ] ] ] ].
+      repeat (eexists; eauto).
+      apply: (corr_term_impl _ _ _ _ _ Hterm) => // l0.
+      move: nth_cat (leqP (size H) l0) =>
+        -> [ /(nth_default _) -> | ]; eauto. }
+    split; eauto.
+    { constructor; rewrite size_mkseq; eauto.
+      move => x ? ? d'.
+      rewrite nth_mkseq => //.
+      apply: corr_term_indir.
+      - by rewrite nth_cat ltnNge leq_addr addKn (nth_map d').
+      - refine (corr_term_impl _ _ _ _ _ (H9 _ _ _) _ _ _ _ _ _) => // l.
+        move: nth_cat (leqP (size H) l) =>
+          -> [ /(nth_default _) -> | ]; eauto. }
+  - move: (IHeval_name1 _ _ _ H4 H9) => [ ? [ ? [ P' [ mu' [ Hheap' [ ] ] ] ] ] ].
+    inversion 1. subst => [ [ ? [ HPmu HQmu ] ] ].
     have Hlt : i < size pts.
-    { move: (leqP (size pts) i) (H3 (c.+1, 0, Var 0)) =>
+    { move: (leqP (size pts) i) (H1 (c.+1, 0, Var 0)) =>
         [ /(nth_default _) -> | // ].
       inversion 1. subst.
-      by move: (PeanoNat.Nat.neq_succ_diag_l _ H11). }
+      by move: (PeanoNat.Nat.neq_succ_diag_l _ H8). }
     have ? : forall d, nth d pts' i = (c, size ts', (nth (0, 0, Var 0) pts' i).2) => [ d | ].
-    { rewrite (surjective_pairing (nth d pts' i)) -H12 -H13 H3.
+    { rewrite (surjective_pairing (nth d pts' i)) -H13 -H14 H1.
       do 2 f_equal. apply: set_nth_default. congruence. }
-    have ? : forall j, j < i -> forall d t1, nth d pts' j = (c, size ts', t1) -> False => [ j Hlt' d | ].
-    { move: (H4 _ Hlt' d).
+    have ? : forall j d t1, nth d pts' j = (c, size ts', t1) -> i <= j => [ j d | ].
+    { move: (H2 j d).
       rewrite
         (surjective_pairing (nth d pts j))
-        (surjective_pairing (nth d pts' j)) H12 H13 => Hcontra.
+        (surjective_pairing (nth d pts' j)) H13 H14 => Hcontra.
       inversion 1. subst.
       apply: Hcontra. f_equal. eauto. }
-    have Hterm'' : corr_term P' mu'
-      (subst (scat ts Var) t0)
+    have Hterm'' : corr_term P' H' mu'
+      (subst (scat (map Loc ls) Var) t0)
       (subst (scat ts' Var) (nth (0, 0, Var 0) pts' i).2).
-    { apply: corr_term_subst => [ | x | ? ].
-      - move: H3 (H14 _ Hlt (0, 0, Var 0)) => -> /corr_term_impl.
-        by apply => [ | /= ? /HPmu -> ].
-      - rewrite !nth_scat H13.
-        case (leqP (size ts) x) => ?.
-        + rewrite !nth_default -?H13; eauto.
-        + eauto using corr_term_impl.
+    { apply: corr_term_subst => [ | x | ? | ? ].
+      - move: H1 (H15 _ Hlt (0, 0, Var 0)) => -> /corr_term_impl
+          /(_ P' (map (omap (rename (addn (c, size ls, t0).1.2))) H')).
+        apply => [ | l | /= ? /HPmu -> ] //=.
+        rewrite !nth_map_heap.
+        move: (nth None H l) (Heaps.eval_name_heap _ _ _ _ H0 l) =>
+          [ ? /(_ _ erefl) -> | ] /=; eauto.
+      - rewrite !nth_scat.
+        case (leqP (size ls) x) => ?.
+        + rewrite !nth_default ?size_map -?H14; eauto.
+        + rewrite (nth_map 0) => //.
+          exact: H17.
+      - rewrite nth_map_heap omap_comp (eq_omap _ _ _ id) ?omap_id => // ?.
+        rewrite /funcomp subst_rename_comp (eq_subst _ _ Var) ?subst_id => //= ?.
+        by rewrite nth_scat nth_default size_map ?leq_addr ?addKn.
       - rewrite subst_rename_comp (eq_subst _ _ Var) ?subst_id => //= ?.
-        by rewrite nth_scat nth_default -H13 ?addKn ?leq_addr. }
-    apply: diverge_name_casematch; eauto.
+        by rewrite nth_scat nth_default -H14 ?addKn ?leq_addr. }
+    move: (IHeval_name2 _ _ _ Hheap' Hterm'') =>
+      [ ? [ ? [ ? [ ? [ ? [ ? [ ? [ ? ? ] ] ] ] ] ] ] ].
+    repeat (eexists; eauto).
+    + move => ? ?.
+      erewrite HPmu; eauto.
+    + move => ? ? ?.
+      erewrite HQmu; eauto.
 Qed.
-    
-Theorem eval_name_complete t2 v2 :
-  eval_name t2 v2 ->
-  forall P mu H1 t1,
-  corr_term P mu t1 t2 ->
+
+Theorem diverge_name_sound :
+  forall H1 t1,
+  Heaps.diverge_name H1 t1 ->
+  forall P mu t2,
   corr_heap P H1 mu ->
-  exists H1' v1,
-  Heaps.eval_name H1 t1 H1' v1 /\
-  exists P' mu',
-  corr_heap P' H1' mu' /\
-  corr_term P' mu' v1 v2 /\
-  ( forall l, P l -> P' l ) /\
-  ( forall l, P l -> mu l = mu' l ).
+  corr_term P H1 mu t1 t2 ->
+  diverge_name t2.
 Proof.
-  induction 1; inversion 1; subst => [ Hheap ].
-  - by move: H4 (Hheap _ H3) => -> [ ? [ ? [ ? [ ? [ ] ] ] ] ].
-  - move: (IHeval_name1 _ _ _ _ H7 Hheap) =>
-      [ H1' [ ? [ ? [ P' [ mu' [ Hheap' [ ] ] ] ] ] ] ].
-    inversion 1; subst => [ [ HP' HPmu' ] ].
-    { by move: H4 (Hheap' _ H3) => -> [ ? [ ? [ ? [ ? [ ] ] ] ] ]. }
-    have Hterm' : corr_term P' mu'
-      (subst (scons t5 Var) t)
-      (subst (scons t2 Var) t0).
-    { apply: corr_term_subst; eauto.
+  cofix diverge_name_sound => H ? Hdiv P mu ? Hheap /unwind_indirection [ ? [ Hrt [ ] ] ].
+  move: (Heaps.diverge_name_red_name_aux _ _ Hrt _ _ _ _ erefl erefl Hdiv).
+  inversion 1; subst.
+  - move => ? /(_ _ erefl) [ /Hheap [ ? [ ] ] ].
+    rewrite H1. inversion 1.
+    subst => [ [ ? [ ? [ -> ? ] ] ] <- ].
+    apply: diverge_name_let. eauto.
+  - inversion 1. subst => ?.
+    apply: diverge_name_appL. eauto.
+  - inversion 1. subst => ?.
+    move: (eval_name_sound _ _ _ _ H1 _ _ _ Hheap H7) =>
+      [ ? [ ? [ P' [ mu' [ Hheap' [ ] ] ] ] ] ].
+    inversion 1. subst => [ [ HP' [ HPmu HQmu ] ] ].
+    have Hterm'' : corr_term P'
+      (rcons H' (Some t2)) mu'
+      (subst (scons (Loc (size H')) Var) t0)
+      (subst (scons t2' Var) t').
+    { apply: corr_term_subst.
+      - ( eapply (corr_term_impl _ _ _ _ _ H6 _
+            (map (omap (rename succn)) (rcons H' (Some t2)))
+            (rename succn \o mu')); eauto ) => l.
+        rewrite !nth_map_heap nth_rcons.
+        case (leqP (size H') l) => [ /(nth_default _) -> //= | ]; eauto.
       - move => [ | ? ] //=.
-        apply: corr_term_impl; eauto.
+        apply: corr_term_indir => /=.
+        + by rewrite nth_rcons ltnn eqxx.
+        + ( apply: corr_term_impl; eauto 2 ) => l /=.
+          move: (nth None H l) (Heaps.eval_name_heap _ _ _ _ H1 l) =>
+            [ ? /(_ _ erefl) | ]; eauto.
+          move: nth_rcons (leqP (size H') l) =>
+            -> [ /(nth_default _) -> // | ? -> ]; eauto.
+      - move => ?.
+        rewrite nth_map_heap omap_comp (eq_omap _ _ _ id) ?omap_id => // ?.
+        by rewrite /funcomp subst_rename_comp (eq_subst _ _ Var) ?subst_id.
       - move => ?.
         by rewrite /funcomp subst_rename_comp (eq_subst _ _ Var) ?subst_id. }
-    move: (IHeval_name2 _ _ _ _ Hterm' Hheap') =>
-      [ ? [ ? [ ? [ ? [ ? [ ? [ ? [ ? ? ] ] ] ] ] ] ] ].
-    repeat (eexists; eauto).
-    move => ? ?.
-    rewrite HPmu'; eauto.
-  - by move: H2 (Hheap _ H0) => -> [ ? [ ? [ ? [ ? [ ] ] ] ] ].
-  - repeat (eexists; eauto).
-  - move: (H3) (Hheap _ H2) => -> [ ? [ ? [ ? [ ? [ ] ] ] ] ].
-    inversion 1. subst => [ Hterm ].
-    move: (IHeval_name _ _ _ _ Hterm Hheap) =>
-      [ ? [ ? [ ? [ ? [ ? [ ? [ ? [ ? ? ] ] ] ] ] ] ] ].
-    repeat (eexists; eauto).
-  - have Hterm' : corr_term
-      (fun l => P l \/ size H1 <= l /\ l - size H1 < size ts0)
-      (fun l => if l < size H1 then mu l else nth (mu l) (map (Let ts) ts) (l - size H1))
-      (subst (scat (mkseq (Loc \o addn (size H1)) (size ts0)) Var) t0)
-      (subst (scat (map (Let ts) ts) Var) t).
+    have Hheap'' : corr_heap P' (rcons H' (Some t2)) mu'.
+    { refine (corr_heap_segment_impl _ _ _ _
+        (corr_heap_ext _ _ _ Hheap' _ _) _ _ _ _ _ _); eauto.
+      move => l.
+      by move: nth_rcons (leqP (size H') l) => -> [ /(nth_default _) -> | ]. }
+    apply: diverge_name_beta; eauto.
+  - inversion 1. subst => ?.
+    have Hterm' : corr_term
+      (fun l => P l \/ size H <= l /\ l - size H < size ts)
+      (H ++ map (Some \o subst (scat (mkseq (Loc \o addn (size H)) (size ts)) Var)) ts)
+      (fun l => if l < size H then mu l else nth (mu l) (map (Let ts') ts') (l - size H))
+      (subst (scat (mkseq (Loc \o addn (size H)) (size ts)) Var) t)
+      (subst (scat (map (Let ts') ts') Var) t').
     { apply: corr_term_subst.
-      - ( eapply (corr_term_impl _ _ _ _ H8 _
-            (rename (addn (size ts0)) \o
-              (fun l => if l < size H1 then mu l else nth (mu l) (map (Let ts) ts) (l - size H1)))); eauto ) => l.
-        by move => /(corr_heap_segment_bound _ _ _ _ Hheap) /= ->.
+      - ( eapply (corr_term_impl _ _ _ _ _ H9 _
+            (map (omap (rename (addn (size ts))))
+              (H ++ map (Some \o subst (scat (mkseq (Loc \o addn (size H)) (size ts)) Var)) ts))
+            (rename (addn (size ts)) \o
+              (fun l => if l < size H then mu l else nth (mu l) (map (Let ts') ts') (l - size H)))); eauto ) => l.
+        + rewrite !nth_map_heap nth_cat.
+          case (leqP (size H) l) => [ /(nth_default _) -> | ] /=; eauto.
+        + by move => /(corr_heap_segment_bound _ _ _ _ Hheap) /= ->.
       - move => x.
         rewrite !nth_scat size_mkseq size_map -H4.
-        case (leqP (size ts0) x) => ?.
+        case (leqP (size ts) x) => ?.
         + rewrite !nth_default ?size_mkseq ?size_map -?H4; eauto.
         + rewrite nth_mkseq => //=.
           apply: corr_term_loc.
@@ -583,135 +678,397 @@ Proof.
             apply: set_nth_default.
             by rewrite size_map -H4.
       - move => ?.
+        rewrite nth_map_heap omap_comp (eq_omap _ _ _ id) ?omap_id => // ?.
+        rewrite /funcomp subst_rename_comp (eq_subst _ _ Var) ?subst_id => // ? /=.
+        by rewrite nth_scat nth_default size_mkseq ?addKn ?leq_addr.
+      - move => ?.
         rewrite /funcomp subst_rename_comp (eq_subst _ _ Var) ?subst_id => //= ?.
         by rewrite nth_scat nth_default size_map -H4 ?addKn ?leq_addr. }
     have Hheap' : corr_heap
-      (fun l => P l \/ size H1 <= l /\ l - size H1 < size ts0)
-      (H1 ++ map (@Some _ \o subst (scat (mkseq (Loc \o addn (size H1)) (size ts0)) Var)) ts0)
-      (fun l => if l < size H1 then mu l else nth (mu l) (map (Let ts) ts) (l - size H1)).
+      (fun l => P l \/ size H <= l /\ l - size H < size ts)
+      (H ++ map (Some \o subst (scat (mkseq (Loc \o addn (size H)) (size ts)) Var)) ts)
+      (fun l => if l < size H then mu l else nth (mu l) (map (Let ts') ts') (l - size H)).
     { apply: corr_heap_segment_union.
       - ( refine (corr_heap_segment_impl _ _ _ _
           (corr_heap_ext _ _ _ Hheap _ _) _ _ _ _ _ _); eauto ) => l.
         + by move => /(corr_heap_segment_bound _ _ _ _ Hheap) ->.
-        + by move: nth_cat (leqP (size H1) l) => -> [ /(nth_default _) -> | ].
+        + by move: nth_cat (leqP (size H) l) => -> [ /(nth_default _) -> | ].
       - move => ? [ Hge Hlt ].
         rewrite nth_cat ltnNge Hge (nth_map (Var 0)) => //=.
         repeat (eexists; eauto).
         + apply: (nth_map (Var 0)).
           by rewrite -H4.
         + apply: corr_term_subst.
-          { ( refine (corr_term_impl _ _ _ _ (H7 _ _ _) _
-              (rename (addn (size ts0)) \o
-                (fun l => if l < size H1 then mu l else nth (mu l) (map (Let ts) ts) (l - size H1))) _ _); eauto ) => l.
-            by move => /(corr_heap_segment_bound _ _ _ _ Hheap) /= ->. }
+          { ( refine (corr_term_impl _ _ _ _ _ (H7 _ _ _) _
+                (map (omap (rename (addn (size ts))))
+                  (H ++ map (Some \o subst (scat (mkseq (Loc \o addn (size H)) (size ts)) Var)) ts))
+                (rename (addn (size ts)) \o
+                  (fun l => if l < size H then mu l else nth (mu l) (map (Let ts') ts') (l - size H))) _ _ _); eauto ) => l.
+            - rewrite !nth_map_heap nth_cat.
+              case (leqP (size H) l) => [ /(nth_default _) -> | ]; eauto.
+            - by move => /(corr_heap_segment_bound _ _ _ _ Hheap) /= ->. }
           { move => x.
-            case (leqP (size ts0) x) => ?.
+            case (leqP (size ts) x) => ?.
             - by rewrite !nth_scat !nth_default ?size_mkseq ?size_map -?H4.
             - rewrite !nth_scat nth_mkseq ?(nth_map (Var 0)) -?H4 => //.
               apply: corr_term_loc.
               + rewrite leq_addr addKn. eauto.
               + by rewrite ltnNge leq_addr (nth_map (Var 0)) addKn -?H4. }
-          { move => l.
+          { move => ?.
+            rewrite nth_map_heap omap_comp (eq_omap _ _ _ id) ?omap_id => // ?.
+            rewrite /funcomp subst_rename_comp (eq_subst _ _ Var) ?subst_id => //= ?.
+            by rewrite nth_scat nth_default size_mkseq ?leq_addr ?addKn. }
+          { move => ?.
             rewrite /funcomp subst_rename_comp (eq_subst _ _ Var) ?subst_id => //= ?.
             by rewrite nth_scat nth_default size_map -H4 ?leq_addr ?addKn. } }
+    apply: diverge_name_let. eauto.
+  - inversion 1. subst => ?.
+    apply: diverge_name_case. eauto.
+  - inversion 1. subst => ?.
+    move: (eval_name_sound _ _ _ _ H1 _ _ _ Hheap H7) => [ ? [ ? [ P' [ mu' [ Hheap' [ ] ] ] ] ] ].
+    inversion 1. subst => [ [ ? [ HPmu HQmu ] ] ].
+    have Hlt : i < size pts.
+    { move: (leqP (size pts) i) (H2 (c.+1, 0, Var 0)) =>
+        [ /(nth_default _) -> | // ].
+      inversion 1. subst.
+      by move: (PeanoNat.Nat.neq_succ_diag_l _ H6). }
+    have ? : forall d, nth d pts' i = (c, size ts', (nth (0, 0, Var 0) pts' i).2) => [ d | ].
+    { rewrite (surjective_pairing (nth d pts' i)) -H11 -H12 H2.
+      do 2 f_equal. apply: set_nth_default. congruence. }
+    have ? : forall j d t1, nth d pts' j = (c, size ts', t1) -> i <= j => [ j d | ].
+    { move: (H3 j d).
+      rewrite
+        (surjective_pairing (nth d pts j))
+        (surjective_pairing (nth d pts' j)) H11 H12 => Hcontra.
+      inversion 1. subst.
+      apply: Hcontra. f_equal. eauto. }
+    have Hterm'' : corr_term P' H' mu'
+      (subst (scat (map Loc ls) Var) t0)
+      (subst (scat ts' Var) (nth (0, 0, Var 0) pts' i).2).
+    { apply: corr_term_subst => [ | x | ? | ? ].
+      - move: H2 (H13 _ Hlt (0, 0, Var 0)) => -> /corr_term_impl
+          /(_ P' (map (omap (rename (addn (size ls)))) H')).
+        apply => [ | l | /= ? /HPmu -> ] //=.
+        rewrite !nth_map_heap.
+        move: (nth None H l) (Heaps.eval_name_heap _ _ _ _ H1 l) =>
+          [ ? /(_ _ erefl) -> | ] /=; eauto.
+      - rewrite !nth_scat.
+        case (leqP (size ls) x) => ?.
+        + rewrite !nth_default ?size_map -?H12; eauto.
+        + rewrite (nth_map 0) => //.
+          eauto using corr_term_impl.
+      - rewrite nth_map_heap omap_comp (eq_omap _ _ _ id) ?omap_id => // ?.
+        rewrite /funcomp subst_rename_comp (eq_subst _ _ Var) ?subst_id => // ? /=.
+        by rewrite nth_scat nth_default size_map ?addKn ?leq_addr.
+      - rewrite subst_rename_comp (eq_subst _ _ Var) ?subst_id => //= ?.
+        by rewrite nth_scat nth_default -H12 ?addKn ?leq_addr. }
+    apply: diverge_name_casematch; eauto.
+Qed.
+    
+Theorem eval_name_complete t2 v2 :
+  eval_name t2 v2 ->
+  forall P mu H1 t1,
+  corr_term P H1 mu t1 t2 ->
+  corr_heap P H1 mu ->
+  exists H1' v1,
+  Heaps.eval_name H1 t1 H1' v1 /\
+  exists P' mu',
+  corr_heap P' H1' mu' /\
+  corr_term P' H1' mu' v1 v2 /\
+  ( forall l, P l -> P' l ) /\
+  ( forall l, P l -> mu l = mu' l ) /\
+  ( forall l t, nth None H1 l = Some t -> mu l = mu' l ).
+Proof.
+  induction 1 => P mu H_ ? /unwind_indirection [ ? [ ? [ ] ] ];
+  inversion 1; subst => Hloc Hheap.
+  - by move: (Hloc _ erefl) => [ /Hheap [ ? [ ? [ ? [ ? [ -> ] ] ] ] ] ].
+  - by move: (Hloc _ erefl) => [ /Hheap [ ? [ ? [ ? [ ? [ -> ] ] ] ] ] ].
+  - move: (IHeval_name1 _ _ _ _ H7 Hheap) => [ H' [ ? [ Hcbn' [ P' [ mu' [ Hheap' [ ] ] ] ] ] ] ].
+    move: (Heaps.eval_name_value _ _ _ _ Hcbn').
+    inversion 1; inversion 1. subst => [ [ ? [ HPmu HQmu ] ] ].
+    have Hterm'' : corr_term P'
+      (rcons H' (Some t4)) mu'
+      (subst (scons (Loc (size H')) Var) t)
+      (subst (scons t2 Var) t0).
+    { apply: corr_term_subst.
+      - ( eapply (corr_term_impl _ _ _ _ _ H9 _
+            (map (omap (rename succn)) (rcons H' (Some t4)))
+            (rename succn \o mu')); eauto ) => l.
+        rewrite !nth_map_heap nth_rcons.
+        case (leqP (size H') l) => [ /(nth_default _) -> //= | ]; eauto.
+      - move => [ | ? ] //=.
+        apply: corr_term_indir => /=.
+        + by rewrite nth_rcons ltnn eqxx.
+        + ( apply: corr_term_impl; eauto 2 ) => l /=.
+          move: nth_rcons  (nth None H_ l)
+            (Heaps.eval_name_heap _ _ _ _ Hcbn' l) =>
+              -> [ ? /(_ _ erefl) | ]; eauto.
+            case (leqP (size H') l) => [ /(nth_default _) -> | ? -> ]; eauto.
+      - move => ?.
+        rewrite nth_map_heap omap_comp (eq_omap _ _ _ id) ?omap_id => // ?.
+        by rewrite /funcomp subst_rename_comp (eq_subst _ _ Var) ?subst_id.
+      - move => ?.
+        by rewrite /funcomp subst_rename_comp (eq_subst _ _ Var) ?subst_id. }
+    have Hheap'' : corr_heap P' (rcons H' (Some t4)) mu'.
+    { refine (corr_heap_segment_impl _ _ _ _
+        (corr_heap_ext _ _ _ Hheap' _ _) _ _ _ _ _ _); eauto.
+      move => l.
+      by move: nth_rcons (leqP (size H') l) => -> [ /(nth_default _) -> | ]. }
+    move: (IHeval_name2 _ _ _ _ Hterm'' Hheap'') =>
+      [ ? [ ? [ ? [ ? [ ? [ ? [ ? [ ? [ HPmu'' HQmu'' ] ] ] ] ] ] ] ] ].
+    repeat (eexists; eauto using Heaps.red_name_multi_eval_name_aux).
+    + move => ? HP.
+      rewrite -HPmu'' => /=; eauto.
+    + move => l t_ HQ.
+      move: nth_rcons (leqP (size H') l)
+        (Heaps.eval_name_heap _ _ _ _ Hcbn' _ _ HQ) (HQmu'' l t_) =>
+        -> [ /(nth_default _) -> // | Hlt ? <- //= ]. eauto.
+  - by move: (Hloc _ erefl) => [ /Hheap [ ? [ ? [ ? [ ? [ -> ] ] ] ] ] ].
+  - by move: (Hloc _ erefl) => [ /Hheap [ ? [ ? [ ? [ ? [ -> ] ] ] ] ] ].
+  - repeat (eexists; eauto using Heaps.red_name_multi_eval_name_aux).
+  - move: (Hloc _ erefl) => [ /Hheap [ ? [ ] ] ].
+    rewrite H1. inversion 1. subst => [ [ ? [ ? [ -> Hterm ] ] ] ].
+    inversion 1. subst.
+    move: (IHeval_name _ _ _ _ Hterm Hheap) => [ ? [ ? [ ? ? ] ] ].
+    repeat (eexists; eauto using Heaps.red_name_multi_eval_name_aux).
+  - move: (Hheap _ H1) => [ ? [ ? [ ? [ ? [ ] ] ] ] ].
+    rewrite H2. inversion 1. subst => [ Hterm ].
+    move: (IHeval_name _ _ _ _ Hterm Hheap) => [ ? [ ? [ ? ? ] ] ].
+    repeat (eexists; eauto using Heaps.red_name_multi_eval_name_aux).
+  - have Hterm' : corr_term
+      (fun l => P l \/ size H_ <= l /\ l - size H_ < size ts0)
+      (H_ ++ map (Some \o subst (scat (mkseq (Loc \o addn (size H_)) (size ts0)) Var)) ts0)
+      (fun l => if l < size H_ then mu l else nth (mu l) (map (Let ts) ts) (l - size H_))
+      (subst (scat (mkseq (Loc \o addn (size H_)) (size ts0)) Var) t0)
+      (subst (scat (map (Let ts) ts) Var) t).
+    { apply: corr_term_subst.
+      - ( eapply (corr_term_impl _ _ _ _ _ H8 _
+            (map (omap (rename (addn (size ts0))))
+              (H_ ++ map (Some \o subst (scat (mkseq (Loc \o addn (size H_)) (size ts0)) Var)) ts0))
+            (rename (addn (size ts0)) \o
+              (fun l => if l < size H_ then mu l else nth (mu l) (map (Let ts) ts) (l - size H_)))); eauto ) => l.
+        + rewrite !nth_map_heap nth_cat.
+          case (leqP (size H_) l) => [ /(nth_default _) -> | ]; eauto.
+        + by move => /(corr_heap_segment_bound _ _ _ _ Hheap) /= ->.
+      - move => x.
+        rewrite !nth_scat size_mkseq size_map.
+        case (leqP (size ts) x) => ?.
+        + rewrite !nth_default ?size_mkseq ?size_map -?H3; eauto.
+        + rewrite nth_mkseq ?H3 => //=.
+          apply: corr_term_loc.
+          * rewrite leq_addr addKn. eauto.
+          * rewrite ltnNge leq_addr addKn.
+            apply: set_nth_default.
+            by rewrite size_map.
+      - move => l.
+        rewrite !nth_map_heap omap_comp (eq_omap _ _ _ id) ?omap_id => // ?.
+        rewrite /funcomp subst_rename_comp (eq_subst _ _ Var) ?subst_id => // ? /=.
+        by rewrite nth_scat nth_default size_mkseq ?addKn ?leq_addr.
+      - move => ?.
+        rewrite /funcomp subst_rename_comp (eq_subst _ _ Var) ?subst_id => //= ?.
+        by rewrite nth_scat nth_default size_map -H3 ?addKn ?leq_addr. }
+    have Hheap' : corr_heap
+      (fun l => P l \/ size H_ <= l /\ l - size H_ < size ts0)
+      (H_ ++ map (Some \o subst (scat (mkseq (Loc \o addn (size H_)) (size ts0)) Var)) ts0)
+      (fun l => if l < size H_ then mu l else nth (mu l) (map (Let ts) ts) (l - size H_)).
+    { apply: corr_heap_segment_union.
+      - ( refine (corr_heap_segment_impl _ _ _ _
+          (corr_heap_ext _ _ _ Hheap _ _) _ _ _ _ _ _); eauto ) => l.
+        + by move => /(corr_heap_segment_bound _ _ _ _ Hheap) ->.
+        + by move: nth_cat (leqP (size H_) l) => -> [ /(nth_default _) -> | ].
+      - move => ? [ Hge Hlt ].
+        rewrite nth_cat ltnNge Hge (nth_map (Var 0)) -?H3 => //=.
+        repeat (eexists; eauto).
+        + apply: (nth_map (Var 0)).
+          by rewrite -H3.
+        + apply: corr_term_subst.
+          { ( refine (corr_term_impl _ _ _ _ _ (H7 _ _ _) _
+                (map (omap (rename (addn (size ts0))))
+                  (H_ ++ map (Some \o subst (scat (mkseq (Loc \o addn (size H_)) (size ts0)) Var)) ts0))
+              (rename (addn (size ts)) \o
+                (fun l => if l < size H_ then mu l else nth (mu l) (map (Let ts) ts) (l - size H_))) _ _ _); eauto ) => l /=.
+            - rewrite !nth_map_heap nth_cat.
+              case (leqP (size H_) l) => [ /(nth_default _) -> | ]; eauto.
+            - by move: H3 => <- /(corr_heap_segment_bound _ _ _ _ Hheap) /= ->. }
+          { move => x.
+            case (leqP (size ts0) x) => ?.
+            - by rewrite !nth_scat !nth_default ?size_mkseq ?size_map -?H3.
+            - rewrite !nth_scat nth_mkseq ?(nth_map (Var 0)) -?H3 => //.
+              apply: corr_term_loc.
+              + rewrite leq_addr addKn. eauto.
+              + by rewrite ltnNge leq_addr (nth_map (Var 0)) addKn -?H3. }
+          { move => l.
+            rewrite nth_map_heap omap_comp (eq_omap _ _ _ id) ?omap_id => // ?.
+            rewrite /funcomp subst_rename_comp (eq_subst _ _ Var) ?subst_id => //= ?.
+            by rewrite nth_scat nth_default size_mkseq ?leq_addr ?addKn. }
+          { move => l.
+            rewrite /funcomp subst_rename_comp (eq_subst _ _ Var) ?subst_id => //= ?.
+            by rewrite nth_scat nth_default size_map -H3 ?leq_addr ?addKn. } }
     move: (IHeval_name _ _ _ _ Hterm' Hheap') =>
-      [ ? [ ? [ ? [ ? [ ? [ ? [ ? [ ? HPmu' ] ] ] ] ] ] ] ].
-    repeat (eexists; eauto).
-    move => ? ?.
-    rewrite -HPmu'; eauto.
-    erewrite corr_heap_segment_bound; eauto.
-  - by move: H2 (Hheap _ H0) => -> [ ? [ ? [ ? [ ? [ ] ] ] ] ].
-  - repeat (eexists; eauto).
-  - by move: H6 (Hheap _ H5) => -> [ ? [ ? [ ? [ ? [ ] ] ] ] ].
-  - move: (IHeval_name1 _ _ _ _ H7 Hheap) => [ ? [ ? [ ? [ P' [ mu' [ Hheap' [ ] ] ] ] ] ] ].
-    inversion 1; subst => [ [ ? HPmu ] ].
-    { by move: H6 (Hheap' _ H5) => -> [ ? [ ? [ ? [ ? [ ] ] ] ] ]. }
+      [ ? [ ? [ ? [ ? [ ? [ ? [ ? [ ? [ HPmu' HQmu' ] ] ] ] ] ] ] ] ].
+    repeat (eexists; eauto using Heaps.red_name_multi_eval_name_aux).
+    + move => ? HP.
+      rewrite -HPmu'; eauto.
+      erewrite corr_heap_segment_bound; eauto.
+    + move => l t_.
+      by move: nth_cat (leqP (size H_) l) (HQmu' l t_) =>
+        -> [ /(nth_default _) -> | ].
+  - by move: (Hloc _ erefl) => [ /Hheap [ ? [ ? [ ? [ ? [ -> ] ] ] ] ] ].
+  - by move: (Hloc _ erefl) => [ /Hheap [ ? [ ? [ ? [ ? [ -> ] ] ] ] ] ].
+  - repeat (eexists; eauto using Heaps.red_name_multi_eval_name_aux).
+  - do 3 (eexists; eauto using Heaps.red_name_multi_eval_name_aux).
+    exists P, mu. split.
+    { move => l /Hheap [ ? [ ] ].
+      move: nth_cat (leqP (size H_) l) =>
+        -> [ /(nth_default _) -> //
+           | ? -> [ ? [ ? [ -> Hterm ] ] ] ].
+      repeat (eexists; eauto).
+      apply: (corr_term_impl _ _ _ _ _ Hterm) => // l0.
+      move: nth_cat (leqP (size H_) l0) =>
+        -> [ /(nth_default _) -> | ]; eauto. }
+    split; eauto.
+    { constructor; rewrite size_mkseq; eauto.
+      move => x ? ? d'.
+      rewrite nth_mkseq => //.
+      apply: corr_term_indir.
+      - by rewrite nth_cat ltnNge leq_addr addKn (nth_map d').
+      - refine (corr_term_impl _ _ _ _ _ (H6 _ _ _) _ _ _ _ _ _) => // l.
+        move: nth_cat (leqP (size H_) l) =>
+          -> [ /(nth_default _) -> | ]; eauto. }
+  - by move: (Hloc _ erefl) => [ /Hheap [ ? [ ? [ ? [ ? [ -> ] ] ] ] ] ].
+  - by move: (Hloc _ erefl) => [ /Hheap [ ? [ ? [ ? [ ? [ -> ] ] ] ] ] ].
+  - move: (IHeval_name1 _ _ _ _ H6 Hheap) => [ H' [ ? [ Hcbn [ P' [ mu' [ Hheap' [ ] ] ] ] ] ] ].
+    move: (Heaps.eval_name_value _ _ _ _ Hcbn). inversion 1; inversion 1.
+    subst => [ [ ? [ HPmu HQmu ] ] ].
     have Hlt : i < size pts.
     { move: (leqP (size pts) i) (H0 (c.+1, 0, Var 0)) =>
         [ /(nth_default _) -> | // ].
       inversion 1. subst.
-      by move: (PeanoNat.Nat.neq_succ_diag_l _ H9). }
-    have ? : forall d, nth d pts0 i = (c, size ts0, (nth (0, 0, Var 0) pts0 i).2) => [ d | ].
-    { rewrite (surjective_pairing (nth d pts0 i)) H11 H13 H0.
+      by move: (PeanoNat.Nat.neq_succ_diag_l _ H5). }
+    have ? : forall d, nth d pts0 i = (c, size ls, (nth (0, 0, Var 0) pts0 i).2) => [ d | ].
+    { rewrite (surjective_pairing (nth d pts0 i)) H11 H0 -H14.
       do 2 f_equal. apply: set_nth_default. congruence. }
-    have ? : forall j, j < i -> forall d t1, nth d pts0 j = (c, size ts0, t1) -> False => [ j Hlt' d | ].
-    { move: (H1 _ Hlt' d).
+    have ? : forall j d t1, nth d pts0 j = (c, size ls, t1) -> i <= j => [ j d | ].
+    { move: (H1 j d).
       rewrite
         (surjective_pairing (nth d pts0 j))
-        (surjective_pairing (nth d pts j)) H11 H13 => Hcontra.
+        (surjective_pairing (nth d pts j)) H11 H14 => Hcontra.
       inversion 1. subst.
       apply: Hcontra. f_equal. eauto. }
-    have Hterm'' : corr_term P' mu'
-      (subst (scat ts0 Var) (nth (0, 0, Var 0) pts0 i).2)
+    have Hterm'' : corr_term P' H' mu'
+      (subst (scat (map Loc ls) Var) (nth (0, 0, Var 0) pts0 i).2)
       (subst (scat ts Var) t0).
-    { apply: corr_term_subst => [ | x | ? ].
-      - move: H8 Hlt => <- /H12 /(_ (0, 0, Var 0)) /corr_term_impl.
-        rewrite H0. by apply => [ | /= ? /HPmu -> ].
-      - rewrite !nth_scat H13.
-        case (leqP (size ts) x) => ?.
-        + rewrite !nth_default -?H13; eauto.
-        + eauto using corr_term_impl.
-      - rewrite subst_rename_comp H11 H0 (eq_subst _ _ Var) ?subst_id => //= ?.
-        by rewrite nth_scat nth_default -H13 ?addKn ?leq_addr. }
+    { apply: corr_term_subst => [ | x | ? | ? ].
+      - move: H7 Hlt => <- /H12 /(_ (0, 0, Var 0)).
+        rewrite H0 => /= /corr_term_impl
+          /(_ P' (map (omap (rename (addn (nth (0, 0, Var 0) pts0 i).1.2))) H')).
+        apply => [ | l | /= ? /HPmu -> ] //=.
+        rewrite !nth_map_heap.
+        move: (nth None H_ l) (Heaps.eval_name_heap _ _ _ _ Hcbn l) =>
+          [ ? /(_ _ erefl) -> | ] /=; eauto.
+      - rewrite !nth_scat.
+        case (leqP (size ls) x) => ?.
+        + rewrite !nth_default ?size_map -?H14; eauto.
+        + rewrite (nth_map 0) => //.
+          exact: H16.
+      - rewrite nth_map_heap omap_comp (eq_omap _ _ _ id) ?omap_id => // ?.
+        rewrite /funcomp subst_rename_comp (eq_subst _ _ Var) ?subst_id ?H11 ?H0 => //= ?.
+        by rewrite nth_scat nth_default size_map H14 ?leq_addr ?addKn.
+      - rewrite subst_rename_comp (eq_subst _ _ Var) ?subst_id ?H11 ?H0 => //= ?.
+        by rewrite nth_scat nth_default -H14 ?leq_addr ?addKn. }
     move: (IHeval_name2 _ _ _ _ Hterm'' Hheap') =>
-      [ ? [ ? [ ? [ ? [ ? [ ? [ ? [ ? ? ] ] ] ] ] ] ] ].
-    repeat (eexists; eauto).
-    move => ? ?.
-    erewrite HPmu; eauto.
+      [ ? [ ? [ ? [ ? [ ? [ ? [ ? [ ? [ ? ? ] ] ] ] ] ] ] ] ].
+    repeat (eexists; eauto using Heaps.red_name_multi_eval_name_aux).
+    + move => ? ?.
+      erewrite HPmu; eauto.
+    + move => ? ? ?.
+      erewrite HQmu; eauto.
 Qed.
 
 Theorem diverge_name_complete :
   forall t2,
   diverge_name t2 ->
   forall P mu H1 t1,
-  corr_term P mu t1 t2 ->
+  corr_term P H1 mu t1 t2 ->
   corr_heap P H1 mu ->
   Heaps.diverge_name H1 t1.
 Proof.
   cofix diverge_name_complete.
-  inversion 1; inversion 1; subst => [ Hheap0 ].
-  - by move: H5 (Hheap0 _ H4) => -> [ ? [ ? [ ? [ ? [ ] ] ] ] ].
-  - apply: Heaps.diverge_name_appL; eauto.
-  - by move: H6 (Hheap0 _ H5) => -> [ ? [ ? [ ? [ ? [ ] ] ] ] ].
-  - move: (eval_name_complete _ _ H0 _ _ _ _ H9 Hheap0) =>
-      [ H1' [ ? [ ? [ P' [ mu' [ Hheap [ ] ] ] ] ] ] ].
-    inversion 1; subst => [ [ ? HPmu ] ].
-    { by move: H5 (Hheap _ H2) => -> [ ? [ ? [ ? [ ? [ ] ] ] ] ]. }
-    have Hterm' : corr_term P' mu'
-      (subst (scons t6 Var) t)
+  inversion 1; inversion 1; subst => [ Hheap ].
+  - apply: Heaps.diverge_name_loc; eauto.
+  - by move: H6 (Hheap _ H5) => -> [ ? [ ? [ ? [ ? [ ] ] ] ] ].
+  - apply: Heaps.diverge_name_appL. eauto.
+  - apply: Heaps.diverge_name_loc; eauto.
+  - by move: H7 (Hheap _ H6) => -> [ ? [ ? [ ? [ ? [ ] ] ] ] ].
+  - move: (eval_name_complete _ _ H0 _ _ _ _ H11 Hheap) =>
+      [ H1' [ ? [ Hcbn [ P' [ mu' [ Hheap' [ ] ] ] ] ] ] ].
+    move: (Heaps.eval_name_value _ _ _ _ Hcbn).
+    inversion 1; inversion 1; subst => [ [ ? [ HPmu HQmu ] ] ].
+    have Hterm' : corr_term
+      P' (rcons H1' (Some t6)) mu'
+      (subst (scons (Loc (size H1')) Var) t)
       (subst (scons t3 Var) t0).
-    { apply: corr_term_subst; eauto.
+    { apply: corr_term_subst.
+      - ( eapply (corr_term_impl _ _ _ _ _ H10 _
+            (map (omap (rename succn)) (rcons H1' (Some t6)))
+            (rename succn \o mu')); eauto ) => l.
+        rewrite !nth_map_heap nth_rcons.
+        case (leqP (size H1') l) => [ /(nth_default _) -> | ] /=; eauto.
       - move => [ | ? ] //=.
-        apply: corr_term_impl; eauto.
+        apply: corr_term_indir => /=.
+        + by rewrite nth_rcons ltnn eqxx.
+        + ( apply: corr_term_impl; eauto 2 ) => l /=.
+          move: nth_rcons (nth None H3 l)
+            (Heaps.eval_name_heap _ _ _ _ Hcbn l) =>
+              -> [ ? /(_ _ erefl) | ]; eauto.
+            case (leqP (size H1') l) => [ /(nth_default _) -> | ? -> ]; eauto.
+      - move => ?.
+        rewrite nth_map_heap omap_comp (eq_omap _ _ _ id) ?omap_id => // ?.
+        by rewrite /funcomp subst_rename_comp (eq_subst _ _ Var) ?subst_id.
       - move => ?.
         by rewrite /funcomp subst_rename_comp (eq_subst _ _ Var) ?subst_id. }
-    apply: Heaps.diverge_name_appabs; eauto.
-  - move: H5 (Hheap0 _ H4) => -> [ ? [ ? [ ? [ ? [ ] ] ] ] ].
-    inversion 1. subst => [ ? ].
+    have Hheap'' : corr_heap P' (rcons H1' (Some t6)) mu'.
+    { refine (corr_heap_segment_impl _ _ _ _
+        (corr_heap_ext _ _ _ Hheap' _ _) _ _ _ _ _ _); eauto.
+      move => l.
+      by move: nth_rcons (leqP (size H1') l) => -> [ /(nth_default _) -> | ]. }
+    apply: Heaps.diverge_name_beta; eauto.
+  - apply: Heaps.diverge_name_loc; eauto.
+  - move: H6 (Hheap _ H5) => -> [ ? [ ? [ ? [ ? []  ] ] ] ].
+    inversion 1. subst => ?.
     apply: Heaps.diverge_name_loc; eauto.
   - have Hterm' : corr_term
       (fun l => P l \/ size H2 <= l /\ l - size H2 < size ts0)
+      (H2 ++ map (@Some _ \o subst (scat (mkseq (Loc \o addn (size H2)) (size ts0)) Var)) ts0)
       (fun l => if l < size H2 then mu l else nth (mu l) (map (Let ts) ts) (l - size H2))
       (subst (scat (mkseq (Loc \o addn (size H2)) (size ts0)) Var) t0)
       (subst (scat (map (Let ts) ts) Var) t).
     { apply: corr_term_subst.
-      - ( eapply (corr_term_impl _ _ _ _ H10 _
+      - ( eapply (corr_term_impl _ _ _ _ _ H12 _
+            (map (omap (rename (addn (size ts0))))
+              (H2 ++ map (@Some _ \o subst (scat (mkseq (Loc \o addn (size H2)) (size ts0)) Var)) ts0))
             (rename (addn (size ts0)) \o
               (fun l => if l < size H2 then mu l else nth (mu l) (map (Let ts) ts) (l - size H2)))); eauto ) => l.
-        by move => /(corr_heap_segment_bound _ _ _ _ Hheap0) /= ->.
+        + rewrite !nth_map_heap nth_cat.
+          case (leqP (size H2) l) => [ /(nth_default _) -> | ]; eauto.
+        + by move => /(corr_heap_segment_bound _ _ _ _ Hheap) /= ->.
       - move => x.
-        rewrite !nth_scat size_mkseq size_map -H6.
+        rewrite !nth_scat size_mkseq size_map -H7.
         case (leqP (size ts0) x) => ?.
-        + rewrite !nth_default ?size_mkseq ?size_map -?H6; eauto.
+        + rewrite !nth_default ?size_mkseq ?size_map -?H7; eauto.
         + rewrite nth_mkseq => //=.
           apply: corr_term_loc.
           * rewrite leq_addr addKn. eauto.
           * rewrite ltnNge leq_addr addKn.
             apply: set_nth_default.
-            by rewrite size_map -H6.
+            by rewrite size_map -H7.
+      - move => ?.
+        rewrite nth_map_heap omap_comp (eq_omap _ _ _ id) ?omap_id => // ?.
+        rewrite /funcomp subst_rename_comp (eq_subst _ _ Var) ?subst_id => // ? /=.
+        by rewrite nth_scat nth_default size_mkseq ?addKn ?leq_addr.
       - move => ?.
         rewrite /funcomp subst_rename_comp (eq_subst _ _ Var) ?subst_id => //= ?.
-        by rewrite nth_scat nth_default size_map -H6 ?addKn ?leq_addr. }
+        by rewrite nth_scat nth_default size_map -H7 ?addKn ?leq_addr. }
     have Hheap' : corr_heap
       (fun l => P l \/ size H2 <= l /\ l - size H2 < size ts0)
       (H2 ++ map (@Some _ \o subst (scat (mkseq (Loc \o addn (size H2)) (size ts0)) Var)) ts0)
@@ -719,61 +1076,78 @@ Proof.
     { apply: corr_heap_segment_union.
       - apply: corr_heap_segment_cat.
         refine (corr_heap_segment_impl _ _ _ _
-          (corr_heap_ext _ _ _ Hheap0 _ _) _ _ _ _ _ _); eauto.
-        by move => ? /(corr_heap_segment_bound _ _ _ _ Hheap0) ->.
+          (corr_heap_ext _ _ _ Hheap _ _) _ _ _ _ _ _); eauto.
+        by move => ? /(corr_heap_segment_bound _ _ _ _ Hheap) ->.
       - move => ? [ Hge Hlt ].
         rewrite nth_cat ltnNge Hge (nth_map (Var 0)) => //=.
         repeat (eexists; eauto).
-        + apply: (nth_map (Var 0)). by rewrite -H6.
+        + apply: (nth_map (Var 0)). by rewrite -H7.
         + apply: corr_term_subst.
-          { ( refine (corr_term_impl _ _ _ _ (H9 _ _ _) _
+          { ( refine (corr_term_impl _ _ _ _ _ (H11 _ _ _) _
+              (map (omap (rename (addn (size ts0))))
+                (H2 ++ map (@Some _ \o subst (scat (mkseq (Loc \o addn (size H2)) (size ts0)) Var)) ts0))
               (rename (addn (size ts0)) \o
-                (fun l => if l < size H2 then mu l else nth (mu l) (map (Let ts) ts) (l - size H2))) _ _); eauto ) => l.
-            by move => /(corr_heap_segment_bound _ _ _ _ Hheap0) /= ->. }
+                (fun l => if l < size H2 then mu l else nth (mu l) (map (Let ts) ts) (l - size H2))) _ _ _); eauto ) => l.
+            - rewrite !nth_map_heap nth_cat.
+              case (leqP (size H2) l) => [ /(nth_default _) -> | ] /=; eauto.
+            - by move => /(corr_heap_segment_bound _ _ _ _ Hheap) /= ->. }
           { move => x.
             case (leqP (size ts0) x) => ?.
-            - by rewrite !nth_scat !nth_default ?size_mkseq ?size_map -?H6.
-            - rewrite !nth_scat nth_mkseq ?(nth_map (Var 0)) -?H6 => //.
+            - by rewrite !nth_scat !nth_default ?size_mkseq ?size_map -?H7.
+            - rewrite !nth_scat nth_mkseq ?(nth_map (Var 0)) -?H7 => //.
               apply: corr_term_loc.
               + rewrite leq_addr addKn. eauto.
-              + by rewrite ltnNge leq_addr (nth_map (Var 0)) addKn -?H6. }
+              + by rewrite ltnNge leq_addr (nth_map (Var 0)) addKn -?H7. }
+          { move => ?.
+            rewrite nth_map_heap omap_comp (eq_omap _ _ _ id) ?omap_id => // ?.
+            rewrite /funcomp subst_rename_comp (eq_subst _ _ Var) ?subst_id => // ? /=.
+            by rewrite nth_scat nth_default size_mkseq ?addKn ?leq_addr. }
           { move => ?.
             rewrite /funcomp subst_rename_comp (eq_subst _ _ Var) ?subst_id => //= ?.
-            by rewrite nth_scat nth_default size_map -H6 ?leq_addr ?addKn. } }
+            by rewrite nth_scat nth_default size_map -H7 ?leq_addr ?addKn. } }
     apply: Heaps.diverge_name_let. eauto.
-  - by move: H5 (Hheap0 _ H4) => -> [ ? [ ? [ ? [ ? [ ] ] ] ] ].
+  - apply: Heaps.diverge_name_loc; eauto.
+  - by move: H6 (Hheap _ H5) => -> [ ? [ ? [ ? [ ? [ ] ] ] ] ].
   - apply: Heaps.diverge_name_case. eauto.
-  - by move: H8 (Hheap0 _ H7) => -> [ ? [ ? [ ? [ ? [ ] ] ] ] ].
-  - move: (eval_name_complete _ _ H0 _ _ _ _ H9 Hheap0) =>
-      [ ? [ ? [ ? [ P' [ mu' [ Hheap' [ ] ] ] ] ] ] ].
-    inversion 1; subst => [ [ ? HPmu ] ].
-    { by move: H7 (Hheap' _ H4) => -> [ ? [ ? [ ? [ ? [ ] ] ] ] ]. }
+  - apply: Heaps.diverge_name_loc; eauto.
+  - by move: H9 (Hheap _ H8) => -> [ ? [ ? [ ? [ ? [ ] ] ] ] ].
+  - move: (eval_name_complete _ _ H0 _ _ _ _ H10 Hheap) =>
+      [ H1' [ ? [ Hcbn [ P' [ mu' [ Hheap' [ ] ] ] ] ] ] ].
+    move: (Heaps.eval_name_value _ _ _ _ Hcbn).
+    inversion 1; inversion 1; subst => [ [ ? [ HPmu HQmu ] ] ].
     have Hlt : i < size pts.
     { move: (leqP (size pts) i) (H1 (c.+1, 0, Var 0)) =>
         [ /(nth_default _) -> | // ].
       inversion 1. subst.
       by move: (PeanoNat.Nat.neq_succ_diag_l _ H8). }
-    have ? : forall d, nth d pts0 i = (c, size ts0, (nth (0, 0, Var 0) pts0 i).2) => [ d | ].
-    { rewrite (surjective_pairing (nth d pts0 i)) H13 H1 H12.
+    have ? : forall d, nth d pts0 i = (c, size ls, (nth (0, 0, Var 0) pts0 i).2) => [ d | ].
+    { rewrite (surjective_pairing (nth d pts0 i)) H15 H1 H17. 
       do 2 f_equal. apply: set_nth_default. congruence. }
-    have ? : forall j, j < i -> forall d t1, nth d pts0 j = (c, size ts0, t1) -> False => [ j Hlt' d | ].
-    { move: (H2 _ Hlt' d).
+    have ? : forall j d t1, nth d pts0 j = (c, size ls, t1) -> i <= j => [ j d | ].
+    { move: (H2 j d).
       rewrite
         (surjective_pairing (nth d pts0 j))
-        (surjective_pairing (nth d pts j)) H13 H12 => Hcontra.
+        (surjective_pairing (nth d pts j)) H15 H17 => Hcontra.
       inversion 1. subst.
       apply: Hcontra. f_equal. eauto. }
-    have Hterm'' : corr_term P' mu'
-      (subst (scat ts0 Var) (nth (0, 0, Var 0) pts0 i).2)
+    have Hterm'' : corr_term P' H1' mu'
+      (subst (scat (map Loc ls) Var) (nth (0, 0, Var 0) pts0 i).2)
       (subst (scat ts Var) t0).
-    { apply: corr_term_subst => [ | x | ? ].
-      - move: H10 Hlt => <- /H14 /(_ (0, 0, Var 0)) /corr_term_impl.
-        rewrite H1. by apply => [ | /= ? /HPmu -> ].
-      - rewrite !nth_scat H12.
+    { apply: corr_term_subst => [ | x | ? | ? ].
+      - move: H11 Hlt => <- /H16 /(_ (0, 0, Var 0)) /corr_term_impl
+          /(_ P' (map (omap (rename (addn (size ls)))) H1')).
+        rewrite H1. apply => [ | l | /= ? /HPmu -> ] //=.
+        rewrite !nth_map_heap H15 H1 H17 => /=.
+        move: (nth None H5 l) (Heaps.eval_name_heap _ _ _ _ Hcbn l) =>
+          [ ? /(_ _ erefl) -> | ] /=; eauto.
+      - rewrite !nth_scat.
         case (leqP (size ts) x) => ?.
-        + rewrite !nth_default -?H12; eauto.
-        + eauto using corr_term_impl.
-      - rewrite subst_rename_comp H13 H1 (eq_subst _ _ Var) ?subst_id => //= ?.
-        by rewrite nth_scat nth_default -H12 ?addKn ?leq_addr. }
+        + rewrite !nth_default ?size_map -?H17; eauto.
+        + rewrite (nth_map 0) ?H17; eauto.
+      - rewrite nth_map_heap omap_comp (eq_omap _ _ _ id) ?omap_id => // ?.
+        rewrite /funcomp subst_rename_comp (eq_subst _ _ Var) ?subst_id => //= ?.
+        by rewrite nth_scat nth_default size_map ?leq_addr ?addKn.
+      - rewrite subst_rename_comp H15 H1 (eq_subst _ _ Var) ?subst_id => //= ?.
+        by rewrite nth_scat nth_default ?addKn ?leq_addr. }
     apply: Heaps.diverge_name_casematch; eauto.
 Qed.
