Clos.v
@@ -1,0 +1,835 @@
+From mathcomp Require Import all_ssreflect.
+
+Require Import Util LambdaLet.
+Require Heaps.
+Require Import Relations.
+
+Inductive env :=
+  | Empty
+  | Cat of env & seq term & env
+  | Mut of seq term & env.
+
+Definition clos := (env * term)%type.
+
+Fixpoint eget E n : option clos :=
+  match E with
+  | Empty => None
+  | Cat E ts E' => nth (eget E' (n - size ts)) (map (Some \o pair E) ts) n
+  | Mut ts E => nth (eget E (n - size ts)) (map (@Some _ \o pair (Mut ts E)) ts) n
+  end.
+
+Inductive eval_name : env -> term -> clos -> Prop :=
+  | eval_name_var E E' t x v :
+      eget E x = Some (E', t) ->
+      eval_name E' t v ->
+      eval_name E (Var x) v
+  | eval_name_app E E' t0 t1 t2 v :
+      eval_name E t1 (E', Abs t0) ->
+      eval_name (Cat E [:: t2] E') t0 v ->
+      eval_name E (App t1 t2) v
+  | eval_name_abs E t0 :
+      eval_name E (Abs t0) (E, Abs t0)
+  | eval_name_let E ts t v :
+      eval_name (Mut ts E) t v ->
+      eval_name E (Let ts t) v
+  | eval_name_ctor E c ts :
+      eval_name E (Cons c ts) (E, Cons c ts)
+  | eval_name_case E E' c i t t0 ts pts v :
+      eval_name E t (E', Cons c ts) ->
+      (forall d, nth d pts i = (c, size ts, t0)) ->
+      (forall j d t0, nth d pts j = (c, size ts, t0) -> i <= j) ->
+      eval_name (Cat E' ts E) t0 v ->
+      eval_name E (Case t pts) v.
+
+CoInductive diverge_name : env -> term -> Prop :=
+  | diverge_name_var E E' t x :
+      eget E x = Some (E', t) ->
+      diverge_name E' t ->
+      diverge_name E (Var x)
+  | diverge_name_appL E t1 t2 :
+      diverge_name E t1 ->
+      diverge_name E (App t1 t2)
+  | diverge_name_beta E E' t0 t1 t2 :
+      eval_name E t1 (E', Abs t0) ->
+      diverge_name (Cat E [:: t2] E') t0 ->
+      diverge_name E (App t1 t2)
+  | diverge_name_let E ts t :
+      diverge_name (Mut ts E) t ->
+      diverge_name E (Let ts t)
+  | diverge_name_case E t pts :
+      diverge_name E t ->
+      diverge_name E (Case t pts)
+  | diverge_name_casematch E E' c i t t0 ts pts :
+      eval_name E t (E', Cons c ts) ->
+      (forall d, nth d pts i = (c, size ts, t0)) ->
+      (forall j d t0, nth d pts j = (c, size ts, t0) -> i <= j) ->
+      diverge_name (Cat E' ts E) t0 ->
+      diverge_name E (Case t pts).
+
+Inductive corr_term (R : nat -> nat -> Prop) H : nat -> term -> term -> Prop :=
+  | corr_term_loc n x l :
+      n <= x ->
+      R l (x - n) ->
+      corr_term R H n (Loc l) (Var x)
+  | corr_term_var n x :
+      x < n ->
+      corr_term R H n (Var x) (Var x)
+  | corr_term_abs n t t' :
+      corr_term R H n.+1 t t' ->
+      corr_term R H n (Abs t) (Abs t')
+  | corr_term_app n t1 t1' t2 t2' :
+      corr_term R H n t1 t1' ->
+      corr_term R H n t2 t2' ->
+      corr_term R H n (App t1 t2) (App t1' t2')
+  | corr_term_let n t t' ts ts' :
+      size ts = size ts' ->
+      ( forall x, x < size ts -> forall d,
+        corr_term R H (size ts + n)
+          (nth d ts x) (nth d ts' x) ) ->
+      corr_term R H (size ts + n) t t' ->
+      corr_term R H n (Let ts t) (Let ts' t')
+  | corr_term_vcons c ls ts ts' :
+      size ls = size ts' ->
+      ( forall x, x < size ls -> forall d,
+        nth None H (nth d ls x) = Some (ts x) ) ->
+      ( forall x, x < size ls -> forall d,
+        corr_term R H 0 (ts x) (nth d ts' x) ) ->
+      corr_term R H 0 (VCons c ls) (Cons c ts')
+  | corr_term_cons n c ts ts' :
+      size ts = size ts' ->
+      ( forall x, x < size ts -> forall d,
+        corr_term R H n (nth d ts x) (nth d ts' x) ) ->
+      corr_term R H n (Cons c ts) (Cons c ts')
+  | corr_term_case n t t' pts pts' :
+      corr_term R H n t t' ->
+      size pts = size pts' ->
+      ( forall x d, (nth d pts x).1 = (nth d pts' x).1 ) ->
+      ( forall x, x < size pts -> forall d,
+        corr_term R H ((nth d pts x).1.2 + n)
+          (nth d pts x).2 (nth d pts' x).2 ) ->
+      corr_term R H n (Case t pts) (Case t' pts').
+
+CoInductive corr_heap H : (nat -> nat -> Prop) -> env -> Prop :=
+  | corr_heap_fold (R : nat -> nat -> Prop) E :
+      ( forall l x, R l x ->
+        exists t1, nth None H l = Some t1 /\
+        exists E' t2, eget E x = Some (E', t2) /\
+        exists R', corr_heap H R' E' /\ corr_term R' H 0 t1 t2 ) ->
+      corr_heap H R E.
+
+Lemma corr_heap_unfold R H E :
+  corr_heap H R E ->
+  forall l x, R l x ->
+  exists t1, nth None H l = Some t1 /\
+  exists E' t2, eget E x = Some (E', t2) /\
+  exists R', corr_heap H R' E' /\ corr_term R' H 0 t1 t2.
+Proof. by inversion 1. Qed.
+
+Hint Constructors eval_name diverge_name corr_term corr_heap.
+
+Lemma corr_term_impl :
+  forall R H n t t',
+  corr_term R H n t t' ->
+  forall (R' : _ -> _ -> Prop) H',
+  (forall l t, R l t -> R' l t) ->
+  (forall l t, nth None H l = Some t -> nth None H' l = Some t) ->
+  corr_term R' H' n t t'.
+Proof. induction 1; eauto. Qed.
+
+Lemma corr_term_subst :
+  forall R H n t t', corr_term R H n t t' ->
+  forall (R' : _ -> _ -> Prop) s m,
+  m <= n ->
+  (forall x, x < m -> s x = Var x) ->
+  (forall x, m <= x -> x < n -> exists l, s x = Loc l) ->
+  (forall l x, n <= x -> R l (x - n) -> R' l (x - m)) ->
+  (forall l x, s x = Loc l -> R' l (x - m)) ->
+  corr_term R' H m (subst s t) t'.
+Proof.
+  have Hs_impl : forall n s m,
+    (forall x, x < m -> s x = Var x) ->
+    (forall x : nat, x < n + m -> upn s n x = Var x).
+  { move => n ? ? Hs x ?.
+    rewrite (eq_upn _ Var) => [ | ? ].
+    - exact: upn_Var.
+    - apply: Hs.
+      by rewrite -(ltn_add2l n) subnKC. }
+  have Hs'_impl: forall ts s m n,
+    (forall x, m <= x -> x < n -> exists l, s x = Loc l) ->
+    (forall x, ts + m <= x -> x < ts + n -> exists l, upn s ts x = Loc l).
+  { move => ts ? m ? Hs' x ? ?.
+    rewrite upn_unfold.
+    have Hleq := leq_trans (leq_addr m _).
+    rewrite ltnNge Hleq => //=.
+    case (Hs' (x - ts)) => [ | | ? -> /= ];
+    [ rewrite -(leq_add2l ts) subnKC
+    | rewrite -(ltn_add2l ts) subnKC | ]; eauto. }
+  have HR_impl: forall ts (R R' : nat -> _) m n,
+    (forall l x, n <= x -> R l (x - n) -> R' l (x - m)) ->
+    (forall l x, ts + n <= x -> R l (x - (ts + n)) -> R' l (x - (ts + m))).
+  { move => ts ? ? ? n HR ? ? ?.
+    rewrite !subnDA. apply: HR.
+    rewrite -(leq_add2l ts) subnKC => //.
+    exact: (leq_trans (leq_addr n _)). }
+  have Hloc_impl : forall ts (R' : nat -> _) s m,
+    (forall l x, s x = Loc l -> R' l (x - m)) ->
+    (forall l x, upn s ts x = Loc l -> R' l (x - (ts + m))).
+  { move => ts ? s m Hloc ? x.
+    rewrite upn_unfold.
+    move: (leqP ts x) subnDA (Hloc^~ (x - ts)) => [ ? -> | // ].
+    case: (s (x - ts)); inversion 2; subst; eauto. }
+  induction 1 => ? ? m Hleq Hs Hs' HR Hloc /=; eauto using leq_trans.
+  - case (leqP m x) => Hlt.
+    + case: (Hs' _ Hlt H0) => ? Heq.
+      rewrite Heq; eauto.
+    + rewrite Hs; eauto.
+  - constructor.
+    apply: IHcorr_term.
+    + exact Hleq.
+    + exact: (Hs_impl 1).
+    + exact: (Hs'_impl 1).
+    + exact: (HR_impl 1).
+    + exact: (Hloc_impl 1).
+  - ( constructor; rewrite size_map ) => // [ x ? d | ];
+    [ rewrite (nth_map d) => //; apply: H2 => // | apply: IHcorr_term ];
+    solve [ by rewrite leq_add2l | exact: Hs_impl | exact: Hs'_impl | exact: HR_impl | exact: Hloc_impl ].
+  - move: leqn0 Hleq => -> /eqP ?. subst.
+    (econstructor; eauto) => ? ? ?.
+    (apply: corr_term_impl; eauto) => l x.
+    move: subn0 (HR l x) => ->. eauto.
+  - constructor; rewrite ?size_map => // ? ? d.
+    rewrite (nth_map d) => //.
+    apply: H2; eauto.
+  - ( constructor; rewrite ?size_map ) => [ | | x d | ? ? d ]; eauto.
+    + case (leqP (size pts) x) => ?.
+      * by rewrite !nth_default ?size_map -?H1.
+      * by rewrite -H2 (nth_map d).
+    + rewrite !(nth_map d) => //.
+      apply: H4 => //=.
+      * by rewrite leq_add2l.
+      * exact: Hs_impl.
+      * exact: Hs'_impl.
+      * exact: HR_impl.
+      * exact: Hloc_impl.
+Qed.
+
+Lemma corr_heap_impl :
+  forall H R E,
+  corr_heap H R E ->
+  forall (R' : nat -> nat -> Prop) H',
+  (forall l x, R' l x -> R l x) ->
+  (forall l t, nth None H l = Some t -> nth None H' l = Some t) ->
+  corr_heap H' R' E.
+Proof.
+  cofix corr_heap_impl.
+  inversion 1.
+  subst => ? ? HR Hext.
+  constructor => ? ? /HR /H1 [ ? [ /Hext -> [ ? [ ? [ -> [ ? [ ? ? ] ] ] ] ] ] ].
+  repeat (eexists; eauto).
+  apply: corr_term_impl; eauto.
+Qed.
+
+Corollary corr_heap_catL H Hd R E :
+  corr_heap H R E ->
+  corr_heap (H ++ Hd) R E.
+Proof.
+  move => /corr_heap_impl.
+  apply => // l.
+  by move: nth_cat (leqP (size H) l) => -> [ /(nth_default _) -> | ].
+Qed.
+
+Corollary corr_heap_rconsL H R E o :
+  corr_heap H R E ->
+  corr_heap (rcons H o) R E.
+Proof. by rewrite -cats1 => /corr_heap_catL. Qed.
+  
+Lemma corr_heap_union H R R' E :
+  corr_heap H R E ->
+  corr_heap H R' E ->
+  corr_heap H (fun l t => R l t \/ R' l t) E.
+Proof.
+  inversion 1. subst.
+  inversion 1. subst.
+  constructor => ? ? [ /H1 | /H3 ]; eauto.
+Qed.
+
+Lemma corr_heap_catR H R E E' ts :
+  corr_heap H R E ->
+  corr_heap H (fun l x => size ts <= x /\ R l (x - size ts)) (Cat E' ts E).
+Proof.
+  inversion 1. subst.
+  constructor => ? ? [ ? /H1 [ ? [ -> /= [ ? [ ? [ -> [ ? [ ? ? ] ] ] ] ] ] ] ].
+  rewrite nth_default ?size_map => //.
+  repeat (eexists; eauto).
+Qed.
+
+Lemma corr_heap_mutR H R E ts :
+  corr_heap H R E ->
+  corr_heap H (fun l x => size ts <= x /\ R l (x - size ts)) (Mut ts E).
+Proof.
+  inversion 1. subst.
+  constructor => ? ? [ ? /H1 [ ? [ -> /= [ ? [ ? [ -> [ ? [ ? ? ] ] ] ] ] ] ] ].
+  rewrite nth_default ?size_map => //.
+  repeat (eexists; eauto).
+Qed.
+
+Theorem eval_name_sound H H' t1 v1 :
+  Heaps.eval_name H t1 H' v1 ->
+  forall R E t2,
+  corr_heap H R E ->
+  corr_term R H 0 t1 t2 ->
+  exists R' E' v2,
+  eval_name E t2 (E', v2) /\
+  corr_heap H' R' E' /\
+  corr_term R' H' 0 v1 v2.
+Proof.
+  induction 1; inversion 1; inversion 1; subst.
+  - move: subn0 H10 => -> /H3 [ ? [ ] ].
+    rewrite H0 => [ ]. inversion 1.
+    subst => [ [ ? [ ? [ ? [ ? [ Hheap Hterm ] ] ] ] ] ].
+    move: (IHeval_name _ _ _ Hheap Hterm) => [ ? [ ? [ ? [ ? [ ? ? ] ] ] ] ].
+    repeat (eexists; eauto).
+  - move: (IHeval_name1 _ _ _ H0 H8) => [ R' [ E' [ ? [ ? [ ] ] ] ] ].
+    inversion 2. subst.
+    have Hterm : corr_term
+      (fun l x => 0 < x /\ R' l (x - 1) \/ l = size H' /\ x = 0) (rcons H' (Some t2)) 0
+      (subst (scons (Loc (size H')) Var) t0) t'.
+    { refine (corr_term_subst _ _ _ _ _
+        (corr_term_impl _ _ _ _ _ H5 _ _ (fun _ _ H => H) _) _ _ _ _ _ _ _ _) =>
+      // [ l | [ | ? ] | ? [ | ? ] | ? [ | ? ] ] //=;
+      rewrite ?addn1 ?subn0 ?subn1 => /=; eauto 3.
+      - by move: nth_rcons (leqP (size H') l) => -> [ /(nth_default _) -> | ].
+      - inversion 1. eauto. }
+    have Hheap : corr_heap (rcons H' (Some t2))
+      (fun l x => 0 < x /\ R' l (x - 1) \/ l = size H' /\ x = 0)
+      (Cat E [:: t2'] E').
+    { apply: corr_heap_union.
+      - apply: corr_heap_rconsL.
+        by refine (corr_heap_catR _ _ _ _ [:: _] _).
+      - constructor => ? ? [ -> -> ] /=.
+        rewrite nth_rcons ltnn eqxx.
+        do 7 (eexists; eauto).
+        + apply: corr_heap_rconsL.
+          refine (corr_heap_impl _ _ _ _ _ _ _ (Heaps.eval_name_heap _ _ _ _ _)); eauto.
+        + (apply: corr_term_impl; eauto 2) =>
+            l ? /(Heaps.eval_name_heap _ _ _ _ H0_).
+          by move: nth_rcons (leqP (size H') l) => -> [ /(nth_default _) -> | ]. }
+    move: (IHeval_name2 _ _ _ Hheap Hterm) =>
+      [ ? [ ? [ ? [ ? [ ? ? ] ] ] ] ].
+    repeat (eexists; eauto).
+  - repeat (eexists; eauto).
+  - have Hterm : corr_term (fun l x =>
+      size ts <= x /\ R l (x - size ts) \/
+      x < size ts /\ l = size H + x)
+      (H ++ map (@Some _ \o
+        subst (scat (mkseq (Loc \o addn (size H)) (size ts)) Var)) ts) 0
+      (subst (scat (mkseq (Loc \o addn (size H)) (size ts)) Var) t) t'.
+    { refine (corr_term_subst _ _ _ _ _
+        (corr_term_impl _ _ _ _ _ H12 _ _ (fun _ _ H => H) _) _ _ _ _ _ _ _ _) =>
+      [ l | | | ? ? | ? ? | ? x ];
+      rewrite ?addn0 ?subn0 ?nth_scat => //=; eauto 3.
+      - by move: nth_cat (leqP (size H) l) => -> [ /(nth_default _) -> | ].
+      - move => ?.
+        rewrite nth_mkseq => //=; eauto.
+      - case (leqP (size ts) x) => ?.
+        + by rewrite !nth_default ?size_mkseq.
+        + rewrite nth_mkseq => //=.
+          inversion 1. subst. eauto. }
+    have Hheap : corr_heap
+      (H ++ map (@Some _ \o
+        subst (scat (mkseq (Loc \o addn (size H)) (size ts)) Var)) ts)
+      (fun l x =>
+        size ts <= x /\ R l (x - size ts) \/
+        x < size ts /\ l = size H + x)
+      (Mut ts' E).
+    { cofix Hheap'.
+      constructor => ? x [ [ ? ? ] | [ ? -> ] /= ].
+      - apply: corr_heap_unfold.
+        + apply: corr_heap_mutR.
+          apply: corr_heap_catL. eauto.
+        + move: H8 => /= <-. eauto.
+      - rewrite nth_cat ltnNge leq_addr addKn !(nth_map (Var 0)) => /=; try congruence.
+        do 7 eexists => /=; eauto.
+        refine (corr_term_subst _ _ _ _ _
+          (corr_term_impl _ _ _ _ _ (H10 _ _ _) _ _ (fun _ _ H => H) _) _ _ _ _ _ _ _ _) =>
+        [ | l | | | ? ? | ? ? | ? y ] //;
+        rewrite ?addn0 ?subn0 ?nth_scat => //; eauto 3.
+        + by move: nth_cat (leqP (size H) l) => -> [ /(nth_default _) -> | ].
+        + move => ?.
+          rewrite nth_mkseq => /=; eauto.
+        + case (leqP (size ts) y) => ?.
+          * by rewrite nth_default ?size_mkseq.
+          * rewrite nth_mkseq => //.
+            inversion 1. subst. eauto. }
+    move: (IHeval_name _ _ _ Hheap Hterm) =>
+      [ ? [ ? [ ? [ ? [ ? ? ] ] ] ] ].
+    repeat (eexists; eauto).
+  - repeat (eexists; eauto).
+  - do 4 (eexists; eauto). split.
+    + refine (corr_heap_impl _ _ _ H0 _ _ (fun _ _ H => H) _) => l.
+      by move: nth_cat (leqP (size H) l) => -> [ /(nth_default _) -> | ].
+    + econstructor; rewrite size_mkseq => // x ? d.
+      * rewrite nth_cat nth_mkseq => //.
+        by rewrite ltnNge leq_addr addKn (nth_map (Var 0)).
+      * rewrite (set_nth_default d) => //.
+        refine (corr_term_impl _ _ _ _ _ (H10 _ _ _) _ _ (fun _ _ H => H) _) => // l.
+        by move: nth_cat (leqP (size H) l) => -> [ /(nth_default _) -> | ].
+  - move: (IHeval_name1 _ _ _ H2 H9) => [ R' [ E' [ ? [ ? [ ] ] ] ] ].
+    inversion 2. subst.
+    have Hlt : i < size pts.
+    { move: (leqP (size pts) i) (H0 (c.+1, 0, Var 0)) =>
+        [ /(nth_default _) -> | // ].
+      inversion 1.
+      by move: (PeanoNat.Nat.neq_succ_diag_l _ H13). }
+    have ? : forall d, nth d pts' i = (c, size ts', (nth (0, 0, Var 0) pts' i).2) => [ d | ].
+    { rewrite (surjective_pairing (nth d pts' i))  -H12 H0 H7 => /=.
+      do 2 f_equal. apply: set_nth_default. congruence. }
+    have ? : forall j d t1, nth d pts' j = (c, size ts', t1) -> i <= j => [ j d | ].
+    { move: (H1 j d).
+      rewrite
+        (surjective_pairing (nth d pts j))
+        (surjective_pairing (nth d pts' j)) -!H12 H7 => Hcontra.
+      inversion 1. subst.
+      apply: Hcontra. f_equal. eauto. }
+    have Hterm' : corr_term
+      (fun l x => size ls <= x /\ R l (x - size ls) \/
+        x < size ls /\ l = nth 0 ls x) H' 0
+      (subst (scat (map Loc ls) Var) t0) (nth (0, 0, Var 0) pts' i).2.
+    { apply: corr_term_subst => [ | | // | ? ? ? | ? ? ? ? | ? x ]; rewrite ?subn0 ?nth_scat.
+      - move: addn0 H0 (H14 _ Hlt (0, 0, Var 0)) => -> -> /= Hterm.
+        refine (corr_term_impl _ _ _ _ _ Hterm _ _ (fun _ _ H => H) (Heaps.eval_name_heap _ _ _ _ _)); eauto.
+      - by [].
+      - rewrite (nth_map 0); eauto.
+      - eauto.
+      - case (leqP (size ls) x) => ?.
+        + by rewrite nth_default ?size_map.
+        + rewrite (nth_map 0) => //. inversion 1. eauto. }
+    have Hheap' : corr_heap H'
+      (fun l x => size ls <= x /\ R l (x - size ls) \/
+        x < size ls /\ l = nth 0 ls x)
+      (Cat E' ts' E).
+    { apply: corr_heap_union.
+      + rewrite H7.
+        apply: corr_heap_catR.
+        refine (corr_heap_impl _ _ _ _ _ _ (fun _ _ H => H)
+          (Heaps.eval_name_heap _ _ _ _ _)); eauto.
+      + constructor => ? ? [ ? -> ] /=.
+        rewrite H8 ?(nth_map (Var 0)) -?H7 => //=.
+        repeat (eexists; eauto). }
+    move: (IHeval_name2 _ _ _ Hheap' Hterm') =>
+      [ ? [ ? [ ? [ ? [ ? ? ] ] ] ] ].
+    repeat (eexists; eauto).
+Qed.
+
+Theorem diverge_name_sound :
+  forall H t1,
+  Heaps.diverge_name H t1 ->
+  forall R E t2,
+  corr_heap H R E ->
+  corr_term R H 0 t1 t2 ->
+  diverge_name E t2.
+Proof.
+  cofix diverge_name_sound.
+  inversion 1; inversion 1; inversion 1; subst.
+  - move: subn0 H14 => -> /H7 [ ? [ ] ].
+    rewrite H2. inversion 1. subst => [ [ ? [ ? [ ? [ ? [ ? ?] ] ] ] ] ].
+    apply: diverge_name_var; eauto.
+  - apply: diverge_name_appL. eauto.
+  - move: (eval_name_sound _ _ _ _ H2 _ _ _ H6 H14) => [ R' [ E' [ ? [ ? [ ] ] ] ] ].
+    inversion 2. subst.
+    have ? : corr_term
+      (fun l x => 0 < x /\ R' l (x - 1) \/ l = size H' /\ x = 0) (rcons H' (Some t3)) 0
+      (subst (scons (Loc (size H')) Var) t0) t'.
+    { refine (corr_term_subst _ _ _ _ _
+        (corr_term_impl _ _ _ _ _ H5 _ _ (fun _ _ H => H) _) _ _ _ _ _ _ _ _) =>
+      // [ l | [ | ? ] | ? [ | ? ] | ? [ | ? ] ] //=;
+      rewrite ?addn1 ?subn0 ?subn1 => /=; eauto 3.
+      - by move: nth_rcons (leqP (size H') l) => -> [ /(nth_default _) -> | ].
+      - inversion 1. eauto. }
+    have Hheap : corr_heap (rcons H' (Some t3))
+      (fun l x => 0 < x /\ R' l (x - 1) \/ l = size H' /\ x = 0)
+      (Cat E [:: t2'] E').
+    { apply: corr_heap_union.
+      - apply: corr_heap_rconsL.
+        by refine (corr_heap_catR _ _ _ _ [:: _] _).
+      - constructor => ? ? [ -> -> ] /=.
+        rewrite nth_rcons ltnn eqxx.
+        do 7 (eexists; eauto).
+        + apply: corr_heap_rconsL.
+          refine (corr_heap_impl _ _ _ _ _ _ _ (Heaps.eval_name_heap _ _ _ _ _)); eauto.
+        + (apply: corr_term_impl; eauto 2) =>
+            l ? /(Heaps.eval_name_heap _ _ _ _ H2).
+          by move: nth_rcons (leqP (size H') l) => -> [ /(nth_default _) -> | ]. }
+    apply: diverge_name_beta; eauto.
+  - have Hterm : corr_term (fun l x =>
+      size ts <= x /\ R l (x - size ts) \/
+      x < size ts /\ l = size H + x)
+      (H ++ map (@Some _ \o
+        subst (scat (mkseq (Loc \o addn (size H)) (size ts)) Var)) ts) 0
+      (subst (scat (mkseq (Loc \o addn (size H)) (size ts)) Var) t) t'.
+    { refine (corr_term_subst _ _ _ _ _
+        (corr_term_impl _ _ _ _ _ H16 _ _ (fun _ _ H => H) _) _ _ _ _ _ _ _ _) =>
+      [ l | | | ? ? | ? ? | ? x ];
+      rewrite ?addn0 ?subn0 ?nth_scat => //=; eauto 3.
+      - by move: nth_cat (leqP (size H) l) => -> [ /(nth_default _) -> | ].
+      - move => ?.
+        rewrite nth_mkseq => //=; eauto.
+      - case (leqP (size ts) x) => ?.
+        + by rewrite !nth_default ?size_mkseq.
+        + rewrite nth_mkseq => //=.
+          inversion 1. subst. eauto. }
+    have Hheap : corr_heap
+      (H ++ map (@Some _ \o
+        subst (scat (mkseq (Loc \o addn (size H)) (size ts)) Var)) ts)
+      (fun l x =>
+        size ts <= x /\ R l (x - size ts) \/
+        x < size ts /\ l = size H + x)
+      (Mut ts' E).
+    { cofix Hheap'.
+      constructor => ? x [ [ ? ? ] | [ ? -> ] /= ].
+      - apply: corr_heap_unfold.
+        + apply: corr_heap_mutR.
+          apply: corr_heap_catL. eauto.
+        + move: H12 => /= <-. eauto.
+      - rewrite nth_cat ltnNge leq_addr addKn !(nth_map (Var 0)) => /=; try congruence.
+        do 7 eexists => /=; eauto.
+        refine (corr_term_subst _ _ _ _ _
+          (corr_term_impl _ _ _ _ _ (H14 _ _ _) _ _ (fun _ _ H => H) _) _ _ _ _ _ _ _ _) =>
+        [ | l | | | ? ? | ? ? | ? y ] //;
+        rewrite ?addn0 ?subn0 ?nth_scat => //; eauto 3.
+        + by move: nth_cat (leqP (size H) l) => -> [ /(nth_default _) -> | ].
+        + move => ?.
+          rewrite nth_mkseq => /=; eauto.
+        + case (leqP (size ts) y) => ?.
+          * by rewrite nth_default ?size_mkseq.
+          * rewrite nth_mkseq => //.
+            inversion 1. subst. eauto. }
+    apply: diverge_name_let. eauto.
+  - apply: diverge_name_case. eauto.
+  - move: (eval_name_sound _ _ _ _ H2 _ _ _ H8 H15) =>
+      [ R' [ E' [ ? [ ? [ ] ] ] ] ].
+    inversion 2. subst.
+    have Hlt : i < size pts.
+    { move: (leqP (size pts) i) (H3 (c.+1, 0, Var 0)) =>
+        [ /(nth_default _) -> | // ].
+      inversion 1.
+      by move: (PeanoNat.Nat.neq_succ_diag_l _ H13). }
+    have ? : forall d, nth d pts' i = (c, size ts', (nth (0, 0, Var 0) pts' i).2) => [ d | ].
+    { rewrite (surjective_pairing (nth d pts' i))  -H18 H3 H7 => /=.
+      do 2 f_equal. apply: set_nth_default. congruence. }
+    have ? : forall j d t1, nth d pts' j = (c, size ts', t1) -> i <= j => [ j d | ].
+    { move: (H4 j d).
+      rewrite
+        (surjective_pairing (nth d pts j))
+        (surjective_pairing (nth d pts' j)) -!H18 H7 => Hcontra.
+      inversion 1. subst.
+      apply: Hcontra. f_equal. eauto. }
+    have Hterm' : corr_term
+      (fun l x => size ls <= x /\ R l (x - size ls) \/
+        x < size ls /\ l = nth 0 ls x) H' 0
+      (subst (scat (map Loc ls) Var) t0) (nth (0, 0, Var 0) pts' i).2.
+    { apply: corr_term_subst => [ | | // | ? ? ? | ? ? ? ? | ? x ]; rewrite ?subn0 ?nth_scat.
+      - move: addn0 H3 (H20 _ Hlt (0, 0, Var 0)) => -> -> /= Hterm.
+        refine (corr_term_impl _ _ _ _ _ Hterm _ _ (fun _ _ H => H) (Heaps.eval_name_heap _ _ _ _ _)); eauto.
+      - by [].
+      - rewrite (nth_map 0); eauto.
+      - eauto.
+      - case (leqP (size ls) x) => ?.
+        + by rewrite nth_default ?size_map.
+        + rewrite (nth_map 0) => //. inversion 1. eauto. }
+    have Hheap' : corr_heap H'
+      (fun l x => size ls <= x /\ R l (x - size ls) \/
+        x < size ls /\ l = nth 0 ls x)
+      (Cat E' ts' E).
+    { apply: corr_heap_union.
+      + rewrite H7.
+        apply: corr_heap_catR.
+        refine (corr_heap_impl _ _ _ _ _ _ (fun _ _ H => H)
+          (Heaps.eval_name_heap _ _ _ _ _)); eauto.
+      + constructor => ? ? [ ? -> ] /=.
+        rewrite H10 ?(nth_map (Var 0)) -?H7 => //=.
+        repeat (eexists; eauto). }
+    apply: diverge_name_casematch; eauto.
+Qed.
+
+Theorem eval_name_complete E t2 c :
+  eval_name E t2 c ->
+  forall R H t1,
+  corr_heap H R E ->
+  corr_term R H 0 t1 t2 ->
+  exists R' H' v1,
+  Heaps.eval_name H t1 H' v1 /\
+  corr_heap H' R' c.1 /\
+  corr_term R' H' 0 v1 c.2.
+Proof.
+  induction 1; inversion 1; inversion 1; subst.
+  - move: subn0 H11 => -> /H3 [ ? [ ? [ ? [ ? [ ] ] ] ] ].
+    rewrite H. inversion 1. subst => [ [ ? [ Hheap Hterm ] ] ].
+    move: (IHeval_name _ _ _ Hheap Hterm) => [ ? [ ? [ ? [ ? [ ? ? ] ] ] ] ].
+    repeat (eexists; eauto).
+  - by [].
+  - move: (IHeval_name1 _ _ _ H2 H11) => /= [ R' [ H' [ ? [ Hcbn [ ] ] ] ] ].
+    inversion 2. subst.
+    have Hterm : corr_term
+      (fun l x => 0 < x /\ R' l (x - 1) \/ l = size H' /\ x = 0) (rcons H' (Some t5)) 0
+      (subst (scons (Loc (size H')) Var) t) t0.
+    { refine (corr_term_subst _ _ _ _ _
+        (corr_term_impl _ _ _ _ _ H8 _ _ (fun _ _ H => H) _) _ _ _ _ _ _ _ _) =>
+      // [ l | [ | ? ] | ? [ | ? ] | ? [ | ? ] ] //=;
+      rewrite ?addn1 ?subn0 ?subn1 => /=; eauto 3.
+      - by move: nth_rcons (leqP (size H') l) => -> [ /(nth_default _) -> | ].
+      - inversion 1. eauto. }
+    have Hheap : corr_heap (rcons H' (Some t5))
+      (fun l x => 0 < x /\ R' l (x - 1) \/ l = size H' /\ x = 0)
+      (Cat E [:: t2] E').
+    { apply: corr_heap_union.
+      - apply: corr_heap_rconsL.
+        by refine (corr_heap_catR _ _ _ _ [:: _] _).
+      - constructor => ? ? [ -> -> ] /=.
+        rewrite nth_rcons ltnn eqxx.
+        do 7 (eexists; eauto).
+        + apply: corr_heap_rconsL.
+          refine (corr_heap_impl _ _ _ _ _ _ _ (Heaps.eval_name_heap _ _ _ _ _)); eauto.
+        + (apply: corr_term_impl; eauto 2) =>
+            l ? /(Heaps.eval_name_heap _ _ _ _ Hcbn).
+          by move: nth_rcons (leqP (size H') l) => -> [ /(nth_default _) -> | ]. }
+    move: (IHeval_name2 _ _ _ Hheap Hterm) => [ ? [ ? [ ? [ ? [ ? ? ] ] ] ] ].
+    repeat (eexists; eauto).
+  - repeat (eexists; eauto).
+  - have Hterm : corr_term (fun l x =>
+      size ts0 <= x /\ R l (x - size ts0) \/
+      x < size ts0 /\ l = size H0 + x)
+      (H0 ++ map (@Some _ \o
+        subst (scat (mkseq (Loc \o addn (size H0)) (size ts0)) Var)) ts0) 0
+      (subst (scat (mkseq (Loc \o addn (size H0)) (size ts0)) Var) t0) t.
+    { refine (corr_term_subst _ _ _ _ _
+        (corr_term_impl _ _ _ _ _ H12 _ _ (fun _ _ H => H) _) _ _ _ _ _ _ _ _) =>
+      [ l | | | ? ? | ? ? | ? x ];
+      rewrite ?addn0 ?subn0 ?nth_scat => //=; eauto 3.
+      - by move: nth_cat (leqP (size H0) l) => -> [ /(nth_default _) -> | ].
+      - move => ?.
+        rewrite nth_mkseq => //=; eauto.
+      - case (leqP (size ts0) x) => ?.
+        + by rewrite !nth_default ?size_mkseq.
+        + rewrite nth_mkseq => //=.
+          inversion 1. subst. eauto. }
+    have Hheap : corr_heap
+      (H0 ++ map (@Some _ \o
+        subst (scat (mkseq (Loc \o addn (size H0)) (size ts0)) Var)) ts0)
+      (fun l x =>
+        size ts0 <= x /\ R l (x - size ts0) \/
+        x < size ts0 /\ l = size H0 + x)
+      (Mut ts E).
+    { cofix Hheap'.
+      constructor => ? x [ [ ? ? ] | [ ? -> ] /= ].
+      - apply: corr_heap_unfold.
+        + apply: corr_heap_mutR.
+          apply: corr_heap_catL. eauto.
+        + move: H8 => /= <-. eauto.
+      - rewrite nth_cat ltnNge leq_addr addKn !(nth_map (Var 0)) => /=; try congruence.
+        do 7 eexists => /=; eauto.
+        refine (corr_term_subst _ _ _ _ _
+          (corr_term_impl _ _ _ _ _ (H11 _ _ _) _ _ (fun _ _ H => H) _) _ _ _ _ _ _ _ _) =>
+        [ | l | | | ? ? | ? ? | ? y ] //;
+        rewrite ?addn0 ?subn0 ?nth_scat => //; eauto 3.
+        + by move: nth_cat (leqP (size H0) l) => -> [ /(nth_default _) -> | ].
+        + move => ?.
+          rewrite nth_mkseq => /=; eauto.
+        + case (leqP (size ts0) y) => ?.
+          * by rewrite nth_default ?size_mkseq.
+          * rewrite nth_mkseq => //.
+            inversion 1. subst. eauto. }
+    move: (IHeval_name _ _ _ Hheap Hterm) =>
+      [ ? [ ? [ ? [ ? [ ? ? ] ] ] ] ].
+    repeat (eexists; eauto).
+  - repeat (eexists; eauto).
+  - do 4 (eexists; eauto). split.
+    + refine (corr_heap_impl _ _ _ H0 _ _ (fun _ _ H => H) _) => l.
+      by move: nth_cat (leqP (size H) l) => -> [ /(nth_default _) -> | ].
+    + econstructor; rewrite size_mkseq => // x ? d.
+      * rewrite nth_cat nth_mkseq => //.
+        by rewrite ltnNge leq_addr addKn (nth_map (Var 0)).
+      * rewrite (set_nth_default d) => //.
+        refine (corr_term_impl _ _ _ _ _ (H10 _ _ _) _ _ (fun _ _ H => H) _) => // l.
+        by move: nth_cat (leqP (size H) l) => -> [ /(nth_default _) -> | ].
+  - move: (IHeval_name1 _ _ _ H4 H11) => [ R' [ H' [ ? [ Hcbn [ ] ] ] ] ].
+    move: (Heaps.eval_name_value _ _ _ _ Hcbn).
+    inversion 1; inversion 2. subst.
+    have Hlt : i < size pts.
+    { move: (leqP (size pts) i) (H0 (c.+1, 0, Var 0)) =>
+        [ /(nth_default _) -> | // ].
+      inversion 1.
+      by move: (PeanoNat.Nat.neq_succ_diag_l _ H9). }
+    have ? : forall d, nth d pts0 i = (c, size ls, (nth (0, 0, Var 0) pts0 i).2) => [ d | ].
+    { rewrite (surjective_pairing (nth d pts0 i))  H15 H0 H14 => /=.
+      do 2 f_equal. apply: set_nth_default. congruence. }
+    have ? : forall j d t1, nth d pts0 j = (c, size ls, t1) -> i <= j => [ j d | ].
+    { move: (H1 j d).
+      rewrite
+        (surjective_pairing (nth d pts0 j))
+        (surjective_pairing (nth d pts j)) !H15 H14 => Hcontra.
+      inversion 1. subst.
+      apply: Hcontra. f_equal. eauto. }
+    have Hterm' : corr_term
+      (fun l x => size ls <= x /\ R l (x - size ls) \/
+        x < size ls /\ l = nth 0 ls x) H' 0
+      (subst (scat (map Loc ls) Var) (nth (0, 0, Var 0) pts0 i).2) t0.
+    { apply: corr_term_subst => [ | | // | ? ? ? | ? ? ? ? | ? x ]; rewrite ?subn0 ?nth_scat.
+      - move: H12 Hlt => <- /H16 /(_ (0, 0, Var 0)).
+        rewrite addn0 H15 H0 => /= Hterm.
+        refine (corr_term_impl _ _ _ _ _ Hterm _ _ (fun _ _ H => H) (Heaps.eval_name_heap _ _ _ _ _)); eauto.
+      - by [].
+      - rewrite (nth_map 0); eauto.
+      - rewrite H14. eauto.
+      - case (leqP (size ls) x) => ?.
+        + by rewrite nth_default ?size_map.
+        + rewrite (nth_map 0) => //. inversion 1. eauto. }
+    have Hheap' : corr_heap H'
+      (fun l x => size ls <= x /\ R l (x - size ls) \/
+        x < size ls /\ l = nth 0 ls x)
+      (Cat E' ts E).
+    { apply: corr_heap_union.
+      + rewrite H14.
+        apply: corr_heap_catR.
+        refine (corr_heap_impl _ _ _ _ _ _ (fun _ _ H => H)
+          (Heaps.eval_name_heap _ _ _ _ _)); eauto.
+      + constructor => ? ? [ ? -> ] /=.
+        rewrite H17 ?(nth_map (Var 0)) -?H14 => //=.
+        repeat (eexists; eauto). }
+    move: (IHeval_name2 _ _ _ Hheap' Hterm') =>
+      [ ? [ ? [ ? [ ? [ ? ? ] ] ] ] ].
+    repeat (eexists; eauto).
+Qed.
+
+Theorem diverge_name_complete :
+  forall E t2,
+  diverge_name E t2 ->
+  forall R H t1,
+  corr_heap H R E ->
+  corr_term R H 0 t1 t2 ->
+  Heaps.diverge_name H t1.
+Proof.
+  cofix diverge_name_complete.
+  inversion 1; inversion 1; inversion 1; subst.
+  - move: subn0 H14 => -> /H6 [ ? [ ? [ ? [ ? [ ] ] ] ] ].
+    rewrite H0. inversion 1. subst => [ [ ? [ ? ? ] ] ].
+    apply: Heaps.diverge_name_loc; eauto.
+  - by [].
+  - apply: Heaps.diverge_name_appL. eauto.
+  - move: (eval_name_complete _ _ _ H0 _ _ _ H5 H14) => [ R' [ H' [ ? [ Hcbn [ ] ] ] ] ].
+    inversion 2. subst.
+    have Hterm : corr_term
+      (fun l x => 0 < x /\ R' l (x - 1) \/ l = size H' /\ x = 0) (rcons H' (Some t6)) 0
+      (subst (scons (Loc (size H')) Var) t) t0.
+    { refine (corr_term_subst _ _ _ _ _
+        (corr_term_impl _ _ _ _ _ H8 _ _ (fun _ _ H => H) _) _ _ _ _ _ _ _ _) =>
+      // [ l | [ | ? ] | ? [ | ? ] | ? [ | ? ] ] //=;
+      rewrite ?addn1 ?subn0 ?subn1 => /=; eauto 3.
+      - by move: nth_rcons (leqP (size H') l) => -> [ /(nth_default _) -> | ].
+      - inversion 1. eauto. }
+    have Hheap : corr_heap (rcons H' (Some t6))
+      (fun l x => 0 < x /\ R' l (x - 1) \/ l = size H' /\ x = 0)
+      (Cat E [:: t3] E').
+    { apply: corr_heap_union.
+      - apply: corr_heap_rconsL.
+        by refine (corr_heap_catR _ _ _ _ [:: _] _).
+      - constructor => ? ? [ -> -> ] /=.
+        rewrite nth_rcons ltnn eqxx.
+        do 7 (eexists; eauto).
+        + apply: corr_heap_rconsL.
+          refine (corr_heap_impl _ _ _ _ _ _ _ (Heaps.eval_name_heap _ _ _ _ _)); eauto.
+        + (apply: corr_term_impl; eauto 2) =>
+            l ? /(Heaps.eval_name_heap _ _ _ _ Hcbn).
+          by move: nth_rcons (leqP (size H') l) => -> [ /(nth_default _) -> | ]. }
+    apply: Heaps.diverge_name_beta; eauto.
+  - have Hterm : corr_term (fun l x =>
+      size ts0 <= x /\ R l (x - size ts0) \/
+      x < size ts0 /\ l = size H3 + x)
+      (H3 ++ map (@Some _ \o
+        subst (scat (mkseq (Loc \o addn (size H3)) (size ts0)) Var)) ts0) 0
+      (subst (scat (mkseq (Loc \o addn (size H3)) (size ts0)) Var) t0) t.
+    { refine (corr_term_subst _ _ _ _ _
+        (corr_term_impl _ _ _ _ _ H15 _ _ (fun _ _ H => H) _) _ _ _ _ _ _ _ _) =>
+      [ l | | | ? ? | ? ? | ? x ];
+      rewrite ?addn0 ?subn0 ?nth_scat => //=; eauto 3.
+      - by move: nth_cat (leqP (size H3) l) => -> [ /(nth_default _) -> | ].
+      - move => ?.
+        rewrite nth_mkseq => //=; eauto.
+      - case (leqP (size ts0) x) => ?.
+        + by rewrite !nth_default ?size_mkseq.
+        + rewrite nth_mkseq => //=.
+          inversion 1. subst. eauto. }
+    have Hheap : corr_heap
+      (H3 ++ map (@Some _ \o
+        subst (scat (mkseq (Loc \o addn (size H3)) (size ts0)) Var)) ts0)
+      (fun l x =>
+        size ts0 <= x /\ R l (x - size ts0) \/
+        x < size ts0 /\ l = size H3 + x)
+      (Mut ts E).
+    { cofix Hheap'.
+      constructor => ? x [ [ ? ? ] | [ ? -> ] /= ].
+      - apply: corr_heap_unfold.
+        + apply: corr_heap_mutR.
+          apply: corr_heap_catL. eauto.
+        + move: H11 => /= <-. eauto.
+      - rewrite nth_cat ltnNge leq_addr addKn !(nth_map (Var 0)) => /=; try congruence.
+        do 7 eexists => /=; eauto.
+        refine (corr_term_subst _ _ _ _ _
+          (corr_term_impl _ _ _ _ _ (H14 _ _ _) _ _ (fun _ _ H => H) _) _ _ _ _ _ _ _ _) =>
+        [ | l | | | ? ? | ? ? | ? y ] //;
+        rewrite ?addn0 ?subn0 ?nth_scat => //; eauto 3.
+        + by move: nth_cat (leqP (size H3) l) => -> [ /(nth_default _) -> | ].
+        + move => ?.
+          rewrite nth_mkseq => /=; eauto.
+        + case (leqP (size ts0) y) => ?.
+          * by rewrite nth_default ?size_mkseq.
+          * rewrite nth_mkseq => //.
+            inversion 1. subst. eauto. }
+    apply: Heaps.diverge_name_let; eauto.
+  - apply: Heaps.diverge_name_case. eauto.
+  - move: (eval_name_complete _ _ _ H0 _ _ _ H7 H14) => [ R' [ H' [ ? [ Hcbn [ ] ] ] ] ].
+    move: (Heaps.eval_name_value _ _ _ _ Hcbn).
+    inversion 1; inversion 2. subst.
+    have Hlt : i < size pts.
+    { move: (leqP (size pts) i) (H1 (c.+1, 0, Var 0)) =>
+        [ /(nth_default _) -> | // ].
+      inversion 1.
+      by move: (PeanoNat.Nat.neq_succ_diag_l _ H9). }
+    have ? : forall d, nth d pts0 i = (c, size ls, (nth (0, 0, Var 0) pts0 i).2) => [ d | ].
+    { rewrite (surjective_pairing (nth d pts0 i))  H18 H1 H13 => /=.
+      do 2 f_equal. apply: set_nth_default. congruence. }
+    have ? : forall j d t1, nth d pts0 j = (c, size ls, t1) -> i <= j => [ j d | ].
+    { move: (H2 j d).
+      rewrite
+        (surjective_pairing (nth d pts0 j))
+        (surjective_pairing (nth d pts j)) !H18 H13 => Hcontra.
+      inversion 1. subst.
+      apply: Hcontra. f_equal. eauto. }
+    have Hterm' : corr_term
+      (fun l x => size ls <= x /\ R l (x - size ls) \/
+        x < size ls /\ l = nth 0 ls x) H' 0
+      (subst (scat (map Loc ls) Var) (nth (0, 0, Var 0) pts0 i).2) t0.
+    { apply: corr_term_subst => [ | | // | ? ? ? | ? ? ? ? | ? x ]; rewrite ?subn0 ?nth_scat.
+      - move: H15 Hlt => <- /H19 /(_ (0, 0, Var 0)).
+        rewrite addn0 H18 H1 => /= Hterm.
+        refine (corr_term_impl _ _ _ _ _ Hterm _ _ (fun _ _ H => H) (Heaps.eval_name_heap _ _ _ _ _)); eauto.
+      - by [].
+      - rewrite (nth_map 0); eauto.
+      - rewrite H13. eauto.
+      - case (leqP (size ls) x) => ?.
+        + by rewrite nth_default ?size_map.
+        + rewrite (nth_map 0) => //. inversion 1. eauto. }
+    have Hheap' : corr_heap H'
+      (fun l x => size ls <= x /\ R l (x - size ls) \/
+        x < size ls /\ l = nth 0 ls x)
+      (Cat E' ts E).
+    { apply: corr_heap_union.
+      + rewrite H13.
+        apply: corr_heap_catR.
+        refine (corr_heap_impl _ _ _ _ _ _ (fun _ _ H => H)
+          (Heaps.eval_name_heap _ _ _ _ _)); eauto.
+      + constructor => ? ? [ ? -> ] /=.
+        rewrite H16 ?(nth_map (Var 0)) -?H13 => //=.
+        repeat (eexists; eauto). }
+    apply: Heaps.diverge_name_casematch; eauto.
+Qed.
